@prefix rdf: <http://www.w3.org/1999/02/22-rdf-syntax-ns#> .
@prefix : <https://example.com#> .
@prefix dc: <http://purl.org/dc/elements/1.1/> .
@prefix owl: <http://www.w3.org/2002/07/owl#> .
@prefix xml: <http://www.w3.org/XML/1998/namespace> .
@prefix xsd: <http://www.w3.org/2001/XMLSchema#> .
@prefix gufo: <http://purl.org/nemo/gufo#> .
@prefix rdfs: <http://www.w3.org/2000/01/rdf-schema#> .
@prefix vann: <http://purl.org/vocab/vann/> .
@prefix terms: <http://purl.org/dc/terms/> .

<https://example.com>
    a owl:Ontology ;
    owl:imports <http://purl.org/nemo/gufo#> .

:AccessDate
    a gufo:SubKind, owl:Class, owl:NamedIndividual ;
    rdfs:comment "Indicates when the dataset was accessed."@en ;
    rdfs:label "AccessDate"@en ;
    rdfs:subClassOf :DataSource .

:Accuracy
    a owl:NamedIndividual, :EvaluationMeasure .

:AccuracySpecifiesSVMEvaluation
    a owl:NamedIndividual, :SpecifiesModelEvaluation ;
    :specifiesInvolvesEvaluationMeasure :Accuracy ;
    :specifiesInvolvesModelEvaluation :SVMEvaluation .

:Addresses
    a gufo:Kind, owl:Class, owl:NamedIndividual ;
    rdfs:comment "Relator that indicates that the Machine Learning Algorithm addresses the goal of the study."@en ;
    rdfs:label "Addresses"@en ;
    rdfs:subClassOf gufo:Relator, [
        a owl:Restriction ;
        owl:minQualifiedCardinality "1"^^xsd:nonNegativeInteger ;
        owl:onClass :Goal ;
        owl:onProperty gufo:mediates
    ], [
        a owl:Restriction ;
        owl:minQualifiedCardinality "1"^^xsd:nonNegativeInteger ;
        owl:onClass :MLAlgorithm ;
        owl:onProperty gufo:mediates
    ] .

:Age_Covid-19
    gufo:hasReifiedQualityValue :Continuous ;
    gufo:isComponentOf :Covid-19 ;
    a owl:NamedIndividual, :Feature ;
    rdfs:comment "AGE Identifies the age of the patient."@en .

:Age_Covid-19Test
    gufo:hasReifiedQualityValue :Continuous ;
    gufo:isComponentOf :Covid-19TestData ;
    a owl:NamedIndividual, :Feature ;
    rdfs:comment "AGE Identifies the age of the patient."@en .

:Age_Covid-19Train
    gufo:hasReifiedQualityValue :Continuous ;
    gufo:isComponentOf :Covid-19TrainData ;
    a owl:NamedIndividual, :Feature ;
    rdfs:comment "AGE Identifies the age of the patient."@en .

:Algorithm
    a gufo:Kind, owl:Class, owl:NamedIndividual ;
    rdfs:comment "The algorithm regardless software implementation. An algorithm can be a machine learning algorithm, a preprocessing algorithm, an evaluation procedure, etc."@en ;
    rdfs:label "Algorithm"@en ;
    rdfs:subClassOf gufo:VariableCollection, [
        a owl:Restriction ;
        owl:onProperty [
            owl:inverseOf gufo:inheresIn
        ] ;
        owl:someValuesFrom :AlgorithmCharacteristic
    ] .

:AlgorithmCharacteristic
    a gufo:Kind, owl:Class, owl:NamedIndividual ;
    rdfs:comment "Characteristics of the Algorithm."@en ;
    rdfs:label "AlgorithmCharacteristic"@en ;
    rdfs:subClassOf gufo:Quality, [
        a owl:Restriction ;
        owl:minQualifiedCardinality "1"^^xsd:nonNegativeInteger ;
        owl:onClass :Algorithm ;
        owl:onProperty gufo:inheresIn
    ] .

:AlgorithmTransparency
    a gufo:SubKind, owl:Class, owl:NamedIndividual ;
    rdfs:comment "Description about how the algorithm usually works."@en ;
    rdfs:label "AlgorithmTransparency"@en ;
    rdfs:subClassOf :AlgorithmCharacteristic .

:Assesses
    a gufo:Kind, owl:Class, owl:NamedIndividual ;
    rdfs:comment "Relator that indicates that the model evaluation assesses the Machine Learning Model."@en ;
    rdfs:label "Assesses"@en ;
    rdfs:subClassOf gufo:Relator, [
        a owl:Restriction ;
        owl:minQualifiedCardinality "1"^^xsd:nonNegativeInteger ;
        owl:onClass :MLModel ;
        owl:onProperty gufo:mediates
    ], [
        a owl:Restriction ;
        owl:minQualifiedCardinality "1"^^xsd:nonNegativeInteger ;
        owl:onClass :ModelEvaluation ;
        owl:onProperty gufo:mediates
    ] .

:Asthma_Covid-19
    gufo:hasReifiedQualityValue :Categorical ;
    gufo:isComponentOf :Covid-19 ;
    a owl:NamedIndividual, :Feature ;
    rdfs:comment "Asthma Identifies if the patient has a diagnosis of asthma."@en .

:Asthma_Covid-19Test
    gufo:hasReifiedQualityValue :Categorical ;
    gufo:isComponentOf :Covid-19TestData ;
    a owl:NamedIndividual, :Feature ;
    rdfs:comment "Asthma Identifies if the patient has a diagnosis of asthma."@en .

:Asthma_Covid-19Test_categories
    gufo:hasQualityValue "1 = Yes , 2 = No"^^xsd:string ;
    gufo:inheresIn :Asthma_Covid-19Test ;
    a owl:NamedIndividual, :Categories .

:Asthma_Covid-19Train
    gufo:hasReifiedQualityValue :Categorical ;
    gufo:isComponentOf :Covid-19TrainData ;
    a owl:NamedIndividual, :Feature ;
    rdfs:comment "Asthma Identifies if the patient has a diagnosis of asthma."@en .

:Asthma_Covid-19Train_1
    gufo:hasQualityValue 174 ;
    gufo:inheresIn :Asthma_Covid-19Train ;
    a owl:NamedIndividual, :CategoryQuantity .

:Asthma_Covid-19Train_2
    gufo:hasQualityValue 6441 ;
    gufo:inheresIn :Asthma_Covid-19Train ;
    a owl:NamedIndividual, :CategoryQuantity .

:Asthma_Covid-19Train_categories
    gufo:hasQualityValue "1 = Yes , 2 = No"^^xsd:string ;
    gufo:inheresIn :Asthma_Covid-19Train ;
    a owl:NamedIndividual, :Categories .

:Asthma_Covid-19_1
    gufo:hasQualityValue "18026"^^xsd:string ;
    gufo:inheresIn :Asthma_Covid-19 ;
    a owl:NamedIndividual, :CategoryQuantity .

:Asthma_Covid-19_2
    gufo:hasQualityValue "546824"^^xsd:string ;
    gufo:inheresIn :Asthma_Covid-19 ;
    a owl:NamedIndividual, :CategoryQuantity .

:Asthma_Covid-19_Null
    gufo:hasQualityValue "1752"^^xsd:string ;
    gufo:inheresIn :Asthma_Covid-19 ;
    a owl:NamedIndividual, :NumberNulls .

:Asthma_Covid-19_categories
    gufo:hasQualityValue "1 = Yes , 2 = No"^^xsd:string ;
    gufo:inheresIn :Asthma_Covid-19 ;
    a owl:NamedIndividual, :Categories .

:COPD_Covid-19
    gufo:hasReifiedQualityValue :Categorical ;
    gufo:isComponentOf :Covid-19 ;
    a owl:NamedIndividual, :Feature ;
    rdfs:comment "COPD Identifies if the patient has a diagnosis of chronic obstructive pulmonary disease (COPD)."@en .

:COPD_Covid-19Test_categories
    gufo:hasQualityValue "1 = Yes , 2 = No"^^xsd:string ;
    gufo:inheresIn :COPD_Covid-19Test_exp1 ;
    a owl:NamedIndividual, :Categories .

:COPD_Covid-19Test_exp1
    gufo:hasReifiedQualityValue :Categorical ;
    gufo:isComponentOf :Covid-19TestData ;
    a owl:NamedIndividual, :Feature ;
    rdfs:comment "COPD Identifies if the patient has a diagnosis of chronic obstructive pulmonary disease (COPD)"@en .

:COPD_Covid-19Train
    gufo:hasReifiedQualityValue :Categorical ;
    gufo:isComponentOf :Covid-19TrainData ;
    a owl:NamedIndividual, :Feature ;
    rdfs:comment "COPD Identifies if the patient has a diagnosis of chronic obstructive pulmonary disease (COPD)."@en .

:COPD_Covid-19Train_1
    gufo:hasQualityValue 105 ;
    gufo:inheresIn :COPD_Covid-19Train ;
    a owl:NamedIndividual, :CategoryQuantity .

:COPD_Covid-19Train_2
    gufo:hasQualityValue 6510 ;
    gufo:inheresIn :COPD_Covid-19Train ;
    a owl:NamedIndividual, :CategoryQuantity .

:COPD_Covid-19Train_categories
    gufo:hasQualityValue "1 = Yes , 2 = No"^^xsd:string ;
    gufo:inheresIn :COPD_Covid-19Train ;
    a owl:NamedIndividual, :Categories .

:COPD_Covid-19_1
    gufo:hasQualityValue 9130 ;
    gufo:inheresIn :COPD_Covid-19 ;
    a owl:NamedIndividual, :CategoryQuantity .

:COPD_Covid-19_2
    gufo:hasQualityValue 555723 ;
    gufo:inheresIn :COPD_Covid-19 ;
    a owl:NamedIndividual, :CategoryQuantity .

:COPD_Covid-19_Null
    gufo:hasQualityValue 1749 ;
    gufo:inheresIn :COPD_Covid-19 ;
    a owl:NamedIndividual, :NumberNulls .

:COPD_Covid-19_categories
    gufo:hasQualityValue "1 = Yes , 2 = No"^^xsd:string ;
    gufo:inheresIn :COPD_Covid-19 ;
    a owl:NamedIndividual, :Categories .

:Calls
    a gufo:Kind, owl:Class, owl:NamedIndividual ;
    rdfs:comment "Relator that indicates that the implementation used to generate results or predictions calls the MLModels, which can act as functions and are executed."@en ;
    rdfs:label "Calls"@en ;
    rdfs:subClassOf gufo:Relator, [
        a owl:Restriction ;
        owl:minQualifiedCardinality "1"^^xsd:nonNegativeInteger ;
        owl:onClass :MLModel ;
        owl:onProperty gufo:mediates
    ], [
        a owl:Restriction ;
        owl:minQualifiedCardinality "1"^^xsd:nonNegativeInteger ;
        owl:onClass :PredictImplementation ;
        owl:onProperty gufo:mediates
    ] .

:Cardiovascular_Covid-19
    gufo:hasReifiedQualityValue :Categorical ;
    gufo:isComponentOf :Covid-19 ;
    a owl:NamedIndividual, :Feature ;
    rdfs:comment "CARDIOVASCULAR Identifies if the patient has a diagnosis of cardiovascular disease."@en .

:Cardiovascular_Covid-19Test
    gufo:hasReifiedQualityValue :Categorical ;
    gufo:isComponentOf :Covid-19TestData ;
    a owl:NamedIndividual, :Feature ;
    rdfs:comment "CARDIOVASCULAR Identifies if the patient has a diagnosis of cardiovascular disease."@en .

:Cardiovascular_Covid-19Test_categories
    gufo:hasQualityValue "1 = Yes , 2 = No"^^xsd:string ;
    gufo:inheresIn :Cardiovascular_Covid-19Test ;
    a owl:NamedIndividual, :Categories .

:Cardiovascular_Covid-19Train
    gufo:hasReifiedQualityValue :Categorical ;
    gufo:isComponentOf :Covid-19TrainData ;
    a owl:NamedIndividual, :Feature ;
    rdfs:comment "CARDIOVASCULAR Identifies if the patient has a diagnosis of cardiovascular disease."@en .

:Cardiovascular_Covid-19Train_1
    gufo:hasQualityValue 132 ;
    gufo:inheresIn :Cardiovascular_Covid-19Train ;
    a owl:NamedIndividual, :CategoryQuantity .

:Cardiovascular_Covid-19Train_2
    gufo:hasQualityValue 6483 ;
    gufo:inheresIn :Cardiovascular_Covid-19Train ;
    a owl:NamedIndividual, :CategoryQuantity .

:Cardiovascular_Covid-19Train_categories
    gufo:hasQualityValue "1 = Yes , 2 = No"^^xsd:string ;
    gufo:inheresIn :Cardiovascular_Covid-19Train ;
    a owl:NamedIndividual, :Categories .

:Cardiovascular_Covid-19_1
    gufo:hasQualityValue 12775 ;
    gufo:inheresIn :Cardiovascular_Covid-19 ;
    a owl:NamedIndividual, :CategoryQuantity .

:Cardiovascular_Covid-19_2
    gufo:hasQualityValue 552005 ;
    gufo:inheresIn :Cardiovascular_Covid-19 ;
    a owl:NamedIndividual, :CategoryQuantity .

:Cardiovascular_Covid-19_Null
    gufo:hasQualityValue 1822 ;
    gufo:inheresIn :Cardiovascular_Covid-19 ;
    a owl:NamedIndividual, :NumberNulls .

:Cardiovascular_Covid-19_categories
    gufo:hasQualityValue "1 = Yes , 2 = No"^^xsd:string ;
    gufo:inheresIn :Cardiovascular_Covid-19 ;
    a owl:NamedIndividual, :Categories .

:Categorical
    a owl:NamedIndividual, :DataType .

:Categories
    a gufo:SubKind, owl:Class, owl:NamedIndividual ;
    rdfs:comment "Categories of a categorical variable."@en ;
    rdfs:label "Categories"@en ;
    rdfs:subClassOf :FeatureCharacteristic .

:CategoryQuantity
    a gufo:SubKind, owl:Class, owl:NamedIndividual ;
    rdfs:comment "Quantity of each category for a categorical variable."@en ;
    rdfs:label "CategoryQuantity"@en ;
    rdfs:subClassOf :FeatureCharacteristic .

:Classification
    a owl:NamedIndividual, :MLTechnique ;
    rdfs:comment "Indicates that the ML algorithm performs classification tasks." .

:ClassificationMetric1
    gufo:hasQualityValue "Accuracy"^^xsd:string ;
    gufo:inheresIn :ClassifyMortality_exp1 ;
    a owl:NamedIndividual, :SuitableMeasurement .

:ClassificationMetric2
    gufo:hasQualityValue "Specificity"^^xsd:string ;
    gufo:inheresIn :ClassifyMortality_exp1 ;
    a owl:NamedIndividual, :SuitableMeasurement .

:ClassificationMetric3
    gufo:hasQualityValue "Sensitivity"^^xsd:string ;
    gufo:inheresIn :ClassifyMortality_exp1 ;
    a owl:NamedIndividual, :SuitableMeasurement .

:ClassificationReport
    a owl:NamedIndividual, :EvaluationProcedure .

:ClassificationReportPython
    dc:creator "Scikit-learn: Machine Learning in Python, Pedregosa et al., JMLR 12, pp. 2825-2830, 2011."^^xsd:string ;
    gufo:isComponentOf :MLWorkflow, :PythonNotebook ;
    a owl:NamedIndividual, :EvaluateModelImplementation ;
    rdfs:comment "Implementation of the classification report containing relevant metrics for classification problems in scikit-learn library to Python."^^xsd:string ;
    :executedBy :EvaluateSVM .

:ClassificationReportPythonFromLibrary
    dc:creator "Scikit-learn: Machine Learning in Python, Pedregosa et al., JMLR 12, pp. 2825-2830, 2011."^^xsd:string ;
    gufo:hasQualityValue "scikit-learn"^^xsd:string ;
    gufo:inheresIn :ClassificationReportPython ;
    a owl:NamedIndividual, :ImplementationLibrary .

:ClassificationReportPythonImplementsClassificationReport
    a owl:NamedIndividual, :Implements ;
    :implementsInvolvesAlgorithm :ClassificationReport ;
    :implementsInvolvesImplementation :ClassificationReportPython .

:ClassifyMortality_exp1
    dc:creator "Patricia"^^xsd:string, """The goal of the experiment 1 is to understand the ML model using the RIPPER rule extractor method. 
The ML model is used to predict mortality of confirmed cases using Epidemiology dataset of tested people for COVID-19 in Mexico."""^^xsd:string ;
    gufo:participatedIn :Experiment1 ;
    a owl:NamedIndividual, :Goal .

:ClassifyMortality_exp2
    gufo:participatedIn :Experiment2 ;
    a owl:NamedIndividual, :Goal .

:CleanData
    a owl:NamedIndividual, :PreprocessingTechnique ;
    rdfs:comment "Indicates that the preprocessing technique is related to cleaning the data." .

:ColumnsSpecifiesRenameColumnSetting
    a owl:NamedIndividual, :SpecifiesParameter ;
    :specifiesInvolvesParameter :RenameColumnParam ;
    :specifiesInvolvesParameterSetting :RenameColumnSetting .

:ContactOtherCovid_Covid-19
    gufo:hasReifiedQualityValue :Categorical ;
    gufo:isComponentOf :Covid-19 ;
    a owl:NamedIndividual, :Feature ;
    rdfs:comment "Identify if the patient had contact with any other case diagnosed with SARS CoV-2."@en .

:ContactOtherCovid_Covid-19_1
    gufo:hasQualityValue 221867 ;
    gufo:inheresIn :ContactOtherCovid_Covid-19 ;
    a owl:NamedIndividual, :CategoryQuantity .

:ContactOtherCovid_Covid-19_2
    gufo:hasQualityValue 169704 ;
    gufo:inheresIn :ContactOtherCovid_Covid-19 ;
    a owl:NamedIndividual, :CategoryQuantity .

:ContactOtherCovid_Covid-19_Null
    gufo:hasQualityValue 175031 ;
    gufo:inheresIn :ContactOtherCovid_Covid-19 ;
    a owl:NamedIndividual, :NumberNulls .

:ContactOtherCovid_Covid-19_categories
    gufo:hasQualityValue "1 = Yes , 2 = No"^^xsd:string ;
    gufo:inheresIn :ContactOtherCovid_Covid-19 ;
    a owl:NamedIndividual, :Categories .

:Continuous
    a owl:NamedIndividual, :DataType .

:Correlates
    a gufo:Kind, owl:Class, owl:NamedIndividual ;
    rdfs:comment "Relator that indicates that two features from the data are mathematically correlated."@en ;
    rdfs:label "Correlates"@en ;
    rdfs:subClassOf gufo:Relator, [
        a owl:Restriction ;
        owl:minQualifiedCardinality "2"^^xsd:nonNegativeInteger ;
        owl:onClass :Feature ;
        owl:onProperty gufo:mediates
    ], [
        a owl:Restriction ;
        owl:onClass :CorrelationCharacteristic ;
        owl:onProperty [
            owl:inverseOf gufo:inheresIn
        ] ;
        owl:qualifiedCardinality "1"^^xsd:nonNegativeInteger
    ] .

:CorrelationCharacteristic
    a gufo:Kind, owl:Class, owl:NamedIndividual ;
    rdfs:comment "Characteristics of the correlations between features."@en ;
    rdfs:label "CorrelationCharacteristic"@en ;
    rdfs:subClassOf gufo:Quality, [
        a owl:Restriction ;
        owl:minQualifiedCardinality "1"^^xsd:nonNegativeInteger ;
        owl:onClass :Correlates ;
        owl:onProperty gufo:inheresIn
    ] .

:CoverageRipperRule01
    gufo:hasQualityValue 102 ;
    gufo:inheresIn :EvaluationRipperRule01 ;
    a owl:NamedIndividual, :ExplanationCoverage .

:CoverageRipperRule02
    gufo:hasQualityValue 30 ;
    gufo:inheresIn :EvaluationRipperRule02 ;
    a owl:NamedIndividual, :ExplanationCoverage .

:CoverageRipperRule03
    gufo:hasQualityValue 13 ;
    gufo:inheresIn :EvaluationRipperRule03 ;
    a owl:NamedIndividual, :ExplanationCoverage .

:CoverageRipperRule04
    gufo:hasQualityValue 165 ;
    gufo:inheresIn :EvaluationRipperRule04 ;
    a owl:NamedIndividual, :ExplanationCoverage .

:CoverageRipperRule05
    gufo:hasQualityValue 76 ;
    gufo:inheresIn :EvaluationRipperRule05 ;
    a owl:NamedIndividual, :ExplanationCoverage .

:CoverageRipperRule06
    gufo:hasQualityValue 184 ;
    gufo:inheresIn :EvaluationRipperRule06 ;
    a owl:NamedIndividual, :ExplanationCoverage .

:CoverageRipperRule07
    gufo:hasQualityValue 29 ;
    gufo:inheresIn :EvaluationRipperRule07 ;
    a owl:NamedIndividual, :ExplanationCoverage .

:CoverageRipperRule08
    gufo:hasQualityValue 53 ;
    gufo:inheresIn :EvaluationRipperRule08 ;
    a owl:NamedIndividual, :ExplanationCoverage .

:CoverageRipperRule09
    gufo:hasQualityValue 22 ;
    gufo:inheresIn :EvaluationRipperRule09 ;
    a owl:NamedIndividual, :ExplanationCoverage .

:CoverageRipperRule10
    gufo:hasQualityValue 15 ;
    gufo:inheresIn :EvaluationRipperRule10 ;
    a owl:NamedIndividual, :ExplanationCoverage .

:CoverageRipperRule11
    gufo:hasQualityValue 10 ;
    gufo:inheresIn :EvaluationRipperRule11 ;
    a owl:NamedIndividual, :ExplanationCoverage .

:CoverageRipperRule12
    gufo:hasQualityValue 13 ;
    gufo:inheresIn :EvaluationRipperRule12 ;
    a owl:NamedIndividual, :ExplanationCoverage .

:CoverageRipperRule13
    gufo:hasQualityValue 16 ;
    gufo:inheresIn :EvaluationRipperRule13 ;
    a owl:NamedIndividual, :ExplanationCoverage .

:CoverageRipperRule14
    gufo:hasQualityValue 13 ;
    gufo:inheresIn :EvaluationRipperRule14 ;
    a owl:NamedIndividual, :ExplanationCoverage .

:CoverageRipperRule15
    gufo:hasQualityValue 28 ;
    gufo:inheresIn :EvaluationRipperRule15 ;
    a owl:NamedIndividual, :ExplanationCoverage .

:CoverageRipperRule16
    gufo:hasQualityValue 82 ;
    gufo:inheresIn :EvaluationRipperRule16 ;
    a owl:NamedIndividual, :ExplanationCoverage .

:CoverageSPLimeExplanation01
    gufo:hasQualityValue 1408 ;
    gufo:inheresIn :EvaluationSPLimeExplanation01 ;
    a owl:NamedIndividual, :ExplanationCoverage .

:CoverageSPLimeExplanation02
    gufo:hasQualityValue 1 ;
    gufo:inheresIn :EvaluationSPLimeExplanation02 ;
    a owl:NamedIndividual, :ExplanationCoverage .

:CoverageSPLimeExplanation03
    gufo:hasQualityValue 1 ;
    gufo:inheresIn :EvaluationSPLimeExplanation03 ;
    a owl:NamedIndividual, :ExplanationCoverage .

:CoverageSPLimeExplanation04
    gufo:hasQualityValue 1 ;
    gufo:inheresIn :EvaluationSPLimeExplanation04 ;
    a owl:NamedIndividual, :ExplanationCoverage .

:CoverageSPLimeExplanation05
    gufo:hasQualityValue 5 ;
    gufo:inheresIn :EvaluationSPLimeExplanation05 ;
    a owl:NamedIndividual, :ExplanationCoverage .

:Covid-19
    gufo:participatedIn :PreprocessCovid ;
    a owl:NamedIndividual, :InputData ;
    rdfs:comment "Epidemiology dataset of tested people for COVID-19 in Mexico"@en .

:Covid-19AccessDate
    gufo:hasQualityValue "22-07-2020"^^xsd:date ;
    gufo:inheresIn :Covid-19 ;
    a owl:NamedIndividual, :AccessDate .

:Covid-19Features
    gufo:hasQualityValue 23 ;
    gufo:inheresIn :Covid-19 ;
    a owl:NamedIndividual, :NumberFeatures .

:Covid-19Instances
    gufo:hasQualityValue 9451 ;
    gufo:inheresIn :Covid-19 ;
    a owl:NamedIndividual, :NumberInstances .

:Covid-19Period
    gufo:hasBeginPointInXSDDate "01-01-2020"^^xsd:date ;
    gufo:hasEndPointInXSDDate "29-06-2020"^^xsd:date ;
    gufo:inheresIn :Covid-19 ;
    a owl:NamedIndividual, :DataPeriod .

:Covid-19SourceName
    gufo:hasQualityValue "Dados Abiertos Mexico"^^xsd:string ;
    gufo:inheresIn :Covid-19 ;
    a owl:NamedIndividual, :SourceName .

:Covid-19TestData
    gufo:participatedIn :EvaluateSVM, :PredictTest ;
    gufo:wasCreatedIn :PreprocessCovid ;
    a owl:NamedIndividual, :TestData ;
    rdfs:comment "Preprocessed test set ."^^xsd:string .

:Covid-19TestFeatures
    gufo:hasQualityValue 17 ;
    gufo:inheresIn :Covid-19TestData ;
    a owl:NamedIndividual, :NumberFeatures .

:Covid-19TestInstances
    gufo:hasQualityValue 2836 ;
    gufo:inheresIn :Covid-19TestData ;
    a owl:NamedIndividual, :NumberInstances .

:Covid-19TestPeriod
    gufo:hasBeginPointInXSDDate "01-06-2020"^^xsd:date ;
    gufo:hasEndPointInXSDDate "02-06-2020"^^xsd:date ;
    gufo:inheresIn :Covid-19TestData ;
    a owl:NamedIndividual, :DataPeriod .

:Covid-19TrainData
    gufo:participatedIn :ExplainSVMLIME, :ExplainSVMRIPPER, :PredictTrain_exp1, :TrainSVM ;
    gufo:wasCreatedIn :PreprocessCovid ;
    a owl:NamedIndividual, :TrainData ;
    rdfs:comment "Preprocessed train set."^^xsd:string .

:Covid-19TrainFeatures
    gufo:hasQualityValue 17 ;
    gufo:inheresIn :Covid-19TrainData ;
    a owl:NamedIndividual, :NumberFeatures .

:Covid-19TrainInstances
    gufo:hasQualityValue 6615 ;
    gufo:inheresIn :Covid-19TrainData ;
    a owl:NamedIndividual, :NumberInstances .

:Covid-19TrainPeriod
    gufo:hasBeginPointInXSDDate "01-06-2020"^^xsd:date ;
    gufo:hasEndPointInXSDDate "02-06-2020"^^xsd:date ;
    gufo:inheresIn :Covid-19TrainData ;
    a owl:NamedIndividual, :DataPeriod .

:Covid-19Website
    gufo:hasQualityValue "https://www.gob.mx/salud/documentos/datos-abiertos-152127"^^xsd:string ;
    gufo:inheresIn :Covid-19 ;
    a owl:NamedIndividual, :Source .

:CovidRes_Covid-19
    gufo:hasReifiedQualityValue :Categorical ;
    gufo:isComponentOf :Covid-19 ;
    a owl:NamedIndividual, :Feature ;
    rdfs:comment "Identifies the result of the analysis of the sample reported by the laboratory of the National Network of Epidemiological Surveillance Laboratories (INDRE, LESP and LAVE). (Catalog of diagnostic results attached)."@en .

:CovidResult_Covid-19_1
    gufo:hasQualityValue 220657 ;
    gufo:inheresIn :CovidRes_Covid-19 ;
    a owl:NamedIndividual, :CategoryQuantity .

:CovidResult_Covid-19_2
    gufo:hasQualityValue 279035 ;
    gufo:inheresIn :CovidRes_Covid-19 ;
    a owl:NamedIndividual, :CategoryQuantity .

:CovidResult_Covid-19_3
    gufo:hasQualityValue 66910 ;
    gufo:inheresIn :CovidRes_Covid-19 ;
    a owl:NamedIndividual, :CategoryQuantity .

:CovidResult_Covid-19_categories
    gufo:hasQualityValue "1=negative, 2=positive, 3=waiting result"^^xsd:string ;
    gufo:inheresIn :CovidRes_Covid-19 ;
    a owl:NamedIndividual, :Categories .

:Data
    a gufo:Kind, owl:Class, owl:NamedIndividual ;
    rdfs:comment "Data are facts and statistics collected together for reference or analysis. They can be images, tables, texts, etc."@en ;
    rdfs:label "Data"@en ;
    rdfs:subClassOf gufo:FunctionalComplex, [
        a owl:Restriction ;
        owl:onProperty [
            owl:inverseOf gufo:inheresIn
        ] ;
        owl:someValuesFrom :DataCharacteristic
    ] .

:DataCharacteristic
    a gufo:Kind, owl:Class, owl:NamedIndividual ;
    rdfs:comment "Characteristics of the data."@en ;
    rdfs:label "DataCharacteristic"@en ;
    rdfs:subClassOf gufo:Quality, [
        a owl:Restriction ;
        owl:minQualifiedCardinality "1"^^xsd:nonNegativeInteger ;
        owl:onClass :Data ;
        owl:onProperty gufo:inheresIn
    ] .

:DataPeriod
    a gufo:SubKind, owl:Class, owl:NamedIndividual ;
    rdfs:comment "Indicates the period of the dataset."@en ;
    rdfs:label "DataPeriod"@en ;
    rdfs:subClassOf :DataCharacteristic .

:DataSource
    a gufo:SubKind, owl:Class, owl:NamedIndividual ;
    rdfs:comment "Indicates the source of the dataset."@en ;
    rdfs:label "DataSource"@en ;
    rdfs:subClassOf :DataCharacteristic .

:DataType
    a gufo:AbstractIndividualType, owl:Class, owl:NamedIndividual ;
    rdfs:comment "Type of data. It can represent the type of data required by the ML Algorithm or the data type of the feature."@en ;
    rdfs:label "DataType"@en ;
    rdfs:subClassOf gufo:QualityValue .

:Date
    a owl:NamedIndividual, :DataType .

:DateDied_Covid-19
    gufo:hasReifiedQualityValue :Date ;
    gufo:isComponentOf :Covid-19 ;
    a owl:NamedIndividual, :Feature ;
    rdfs:comment "Identifies the date the patient died."@en .

:DateSystem_Covid-19
    gufo:hasReifiedQualityValue :Date ;
    gufo:isComponentOf :Covid-19 ;
    a owl:NamedIndividual, :Feature ;
    rdfs:comment "The database is fed daily, this variable allows identifying the date of the last update."@en .

:DeathCorrelatesAge
    a owl:NamedIndividual, :Correlates ;
    :correlates :Age_Covid-19Train, :Death_Covid-19Train .

:DeathCorrelatesAgeValue
    gufo:hasQualityValue 0.355090 ;
    gufo:inheresIn :DeathCorrelatesAge ;
    a owl:NamedIndividual, :CorrelationCharacteristic .

:DeathCorrelatesHospitalized
    a owl:NamedIndividual, :Correlates ;
    :correlates :Death_Covid-19Train, :PatientType_Covid-19Train .

:DeathCorrelatesHospitalizedValue
    gufo:hasQualityValue 0.489923 ;
    gufo:inheresIn :DeathCorrelatesHospitalized ;
    a owl:NamedIndividual, :CorrelationCharacteristic .

:Death_Covid-19Test
    gufo:hasReifiedQualityValue :Categorical ;
    gufo:isComponentOf :Covid-19TestData ;
    a owl:NamedIndividual, :Feature ;
    rdfs:comment "Indicates if the patient died or recovered."@en .

:Death_Covid-19Test_categories
    gufo:hasQualityValue "1 = Yes , 0 = No"^^xsd:string ;
    gufo:inheresIn :Death_Covid-19Test ;
    a owl:NamedIndividual, :Categories .

:Death_Covid-19Train
    gufo:hasReifiedQualityValue :Categorical ;
    gufo:isComponentOf :Covid-19TrainData ;
    a owl:NamedIndividual, :Feature ;
    rdfs:comment "Indicates if the patient died or recovered."@en .

:Death_Covid-19Train_1
    gufo:hasQualityValue 81 ;
    gufo:inheresIn :Death_Covid-19Train ;
    a owl:NamedIndividual, :CategoryQuantity .

:Death_Covid-19Train_2
    gufo:hasQualityValue 6534 ;
    gufo:inheresIn :Death_Covid-19Train ;
    a owl:NamedIndividual, :CategoryQuantity .

:Death_Covid-19Train_categories
    gufo:hasQualityValue "1 = Yes , 0 = No"^^xsd:string ;
    gufo:inheresIn :Death_Covid-19Train ;
    a owl:NamedIndividual, :Categories .

:DecisionTree
    a owl:NamedIndividual, :ExplanationFormat ;
    rdfs:comment "Indicates that the explainable method generates explanations in the format of decision trees." .

:DiabetesCorrelatesICU
    a owl:NamedIndividual, :Correlates ;
    :correlates :Diabetes_Covid-19Train, :ICU_Covid-19Train .

:DiabetesCorrelatesICUValue
    gufo:hasQualityValue 0.245985 ;
    gufo:inheresIn :DiabetesCorrelatesICU ;
    a owl:NamedIndividual, :CorrelationCharacteristic .

:DiabetesCorrelatesPneumonia
    a owl:NamedIndividual, :Correlates ;
    :correlates :Diabetes_Covid-19Train, :Pneumonia_Covid-19Train .

:DiabetesCorrelatesPneumoniaValue
    gufo:hasQualityValue 0.212427 ;
    gufo:inheresIn :DiabetesCorrelatesPneumonia ;
    a owl:NamedIndividual, :CorrelationCharacteristic .

:Diabetes_Covid-19
    gufo:hasReifiedQualityValue :Categorical ;
    gufo:isComponentOf :Covid-19 ;
    a owl:NamedIndividual, :Feature ;
    rdfs:comment "DIABETES Identifies if the patient has a diagnosis of diabetes."@en .

:Diabetes_Covid-19PTrain_categories
    gufo:hasQualityValue "1 = Yes , 2 = No"^^xsd:string ;
    gufo:inheresIn :Diabetes_Covid-19Train ;
    a owl:NamedIndividual, :Categories .

:Diabetes_Covid-19Test
    gufo:hasReifiedQualityValue :Categorical ;
    gufo:isComponentOf :Covid-19TestData ;
    a owl:NamedIndividual, :Feature ;
    rdfs:comment "DIABETES Identifies if the patient has a diagnosis of diabetes."@en .

:Diabetes_Covid-19Test_categories
    gufo:hasQualityValue "1 = Yes , 2 = No"^^xsd:string ;
    gufo:inheresIn :Diabetes_Covid-19Test ;
    a owl:NamedIndividual, :Categories .

:Diabetes_Covid-19Train
    gufo:hasReifiedQualityValue :Categorical ;
    gufo:isComponentOf :Covid-19TrainData ;
    a owl:NamedIndividual, :Feature ;
    rdfs:comment "DIABETES Identifies if the patient has a diagnosis of diabetes."@en .

:Diabetes_Covid-19Train_1
    gufo:hasQualityValue 956 ;
    gufo:inheresIn :Diabetes_Covid-19Train ;
    a owl:NamedIndividual, :CategoryQuantity .

:Diabetes_Covid-19Train_2
    gufo:hasQualityValue 5659 ;
    gufo:inheresIn :Diabetes_Covid-19Train ;
    a owl:NamedIndividual, :CategoryQuantity .

:Diabetes_Covid-19_1
    gufo:hasQualityValue 70831 ;
    gufo:inheresIn :Diabetes_Covid-19 ;
    a owl:NamedIndividual, :CategoryQuantity .

:Diabetes_Covid-19_2
    gufo:hasQualityValue 493790 ;
    gufo:inheresIn :Diabetes_Covid-19 ;
    a owl:NamedIndividual, :CategoryQuantity .

:Diabetes_Covid-19_Null
    gufo:hasQualityValue 1981 ;
    gufo:inheresIn :Diabetes_Covid-19 ;
    a owl:NamedIndividual, :NumberNulls .

:Diabetes_Covid-19_categories
    gufo:hasQualityValue "1 = Yes , 2 = No"^^xsd:string ;
    gufo:inheresIn :Diabetes_Covid-19 ;
    a owl:NamedIndividual, :Categories .

:DimensionalityReduction
    a owl:NamedIndividual, :PreprocessingTechnique ;
    rdfs:comment "Indicates that the preprocessing technique is related to reduce the dimensionality of the data." .

:Discrete
    a owl:NamedIndividual, :DataType .

:DropColumn
    gufo:hasReifiedQualityValue :CleanData ;
    a owl:NamedIndividual, :PreprocessingAlgorithm ;
    rdfs:comment "Remove columns from the dataframe."@en .

:DropColumnsParam
    a owl:NamedIndividual, :Parameter ;
    rdfs:comment "Columns of the dataset to be dropped."@en .

:EntryDate_Covid-19
    gufo:hasReifiedQualityValue :Date ;
    gufo:isComponentOf :Covid-19 ;
    a owl:NamedIndividual, :Feature ;
    rdfs:comment "Identifies the date of the patient's admission to the care unit."@en .

:EvaluateExplanation
    a gufo:EventType, owl:Class, owl:NamedIndividual ;
    rdfs:comment "Specific type of operation that focus on evaluating the explanations generated by the Explain operation."@en ;
    rdfs:label "EvaluateExplanation"@en ;
    rdfs:subClassOf :Operation, [
        a owl:Restriction ;
        owl:minQualifiedCardinality "1"^^xsd:nonNegativeInteger ;
        owl:onClass :EvaluateExplanationImplementation ;
        owl:onProperty [
            owl:inverseOf gufo:participatedIn
        ]
    ], [
        a owl:Restriction ;
        owl:onClass :Explain ;
        owl:onProperty gufo:historicallyDependsOn ;
        owl:qualifiedCardinality "1"^^xsd:nonNegativeInteger
    ], [
        a owl:Restriction ;
        owl:onClass :ExplanationEvaluation ;
        owl:onProperty [
            owl:inverseOf gufo:wasCreatedIn
        ] ;
        owl:qualifiedCardinality "1"^^xsd:nonNegativeInteger
    ] .

:EvaluateExplanationImplementation
    a gufo:SubKind, owl:Class, owl:NamedIndividual ;
    rdfs:comment "Specific type of implementation that implements the evaluation of the explanation."@en ;
    rdfs:label "EvaluateExplanationImplementation"@en ;
    rdfs:subClassOf :Implementation .

:EvaluateLIMEPython
    gufo:isComponentOf :ExplainWorfklow_exp2, :PythonNotebook ;
    a owl:NamedIndividual, :EvaluateExplanationImplementation ;
    :executedBy :EvaluateSPLIME .

:EvaluateModel
    a gufo:EventType, owl:Class, owl:NamedIndividual ;
    rdfs:comment "Specific type of operation that focus on evaluating the ML Model. It executes the implementation of the evaluation procedure, generating the values for the measurements that assess the ML Model."@en ;
    rdfs:label "EvaluateModel"@en ;
    rdfs:subClassOf :Operation, [
        a owl:Restriction ;
        owl:onProperty [
            owl:inverseOf gufo:participatedIn
        ] ;
        owl:someValuesFrom :Result
    ], [
        a owl:Restriction ;
        owl:onProperty [
            owl:inverseOf gufo:participatedIn
        ] ;
        owl:someValuesFrom :TestData
    ], [
        a owl:Restriction ;
        owl:minQualifiedCardinality "1"^^xsd:nonNegativeInteger ;
        owl:onClass :EvaluateModelImplementation ;
        owl:onProperty [
            owl:inverseOf gufo:participatedIn
        ]
    ], [
        a owl:Restriction ;
        owl:onClass :Predict ;
        owl:onProperty gufo:historicallyDependsOn ;
        owl:qualifiedCardinality "1"^^xsd:nonNegativeInteger
    ], [
        a owl:Restriction ;
        owl:onClass :ModelEvaluation ;
        owl:onProperty [
            owl:inverseOf gufo:wasCreatedIn
        ] ;
        owl:qualifiedCardinality "1"^^xsd:nonNegativeInteger
    ] .

:EvaluateModelHasMeasureAccuracy
    a owl:NamedIndividual, :HasMeasure ;
    :hasMeasureInvolvesEvaluateModelImplementation :ClassificationReportPython ;
    :hasMeasureInvolvesMeasure :Accuracy .

:EvaluateModelHasMeasureSensitivity
    a owl:NamedIndividual, :HasMeasure ;
    :hasMeasureInvolvesEvaluateModelImplementation :ClassificationReportPython ;
    :hasMeasureInvolvesMeasure :Sensitivity .

:EvaluateModelHasMeasureSpecificity
    a owl:NamedIndividual, :HasMeasure ;
    :hasMeasureInvolvesEvaluateModelImplementation :ClassificationReportPython ;
    :hasMeasureInvolvesMeasure :Specificity .

:EvaluateModelImplementation
    a gufo:SubKind, owl:Class, owl:NamedIndividual ;
    rdfs:comment "Specific type of implementation that implements the evaluation procedure."@en ;
    rdfs:label "EvaluateModelImplementation"@en ;
    rdfs:subClassOf :Implementation .

:EvaluateRIPPER
    dc:creator "Patricia"^^xsd:string ;
    gufo:historicallyDependsOn :ExplainSVMRIPPER ;
    gufo:isEventProperPartOf :ExplainWorkflow_exec_exp1 ;
    a owl:NamedIndividual, :EvaluateExplanation ;
    rdfs:comment "Evaluate the explanations (rules) generated using RIPPER, regarding coverage of the rules and trustworthiness."^^xsd:string .

:EvaluateRipperPython
    dc:creator "Patricia"^^xsd:string ;
    gufo:isComponentOf :ExplainWorkflow_exp1, :PythonNotebook ;
    a owl:NamedIndividual, :EvaluateExplanationImplementation ;
    rdfs:comment "Manual implementation to evaluate the explanations generated by the RIPPER method. The implementation evaluates coverage of the rules and accuracy of the rules to the test set."^^xsd:string ;
    :executedBy :EvaluateRIPPER .

:EvaluateSPLIME
    gufo:historicallyDependsOn :ExplainSVMLIME ;
    gufo:isEventProperPartOf :ExplainWorkflow_exec_exp2 ;
    a owl:NamedIndividual, :EvaluateExplanation .

:EvaluateSVM
    gufo:historicallyDependsOn :PredictTest ;
    gufo:isEventProperPartOf :MLWorkflow_exec ;
    a owl:NamedIndividual, :EvaluateModel ;
    rdfs:comment "Evaluate the fitted SVM ML model according to the evaluation procedures and measures."^^xsd:string .

:EvaluatesExplanationComponent
    a gufo:Kind, owl:Class, owl:NamedIndividual ;
    rdfs:comment "Relator that indicates that the component of the explanation evaluation evaluates explanation components (e.g., coverage)."@en ;
    rdfs:label "EvaluatesExplanationComponent"@en ;
    rdfs:subClassOf gufo:Relator, [
        a owl:Restriction ;
        owl:minQualifiedCardinality "1"^^xsd:nonNegativeInteger ;
        owl:onClass :ExplanationComponent ;
        owl:onProperty gufo:mediates
    ], [
        a owl:Restriction ;
        owl:minQualifiedCardinality "1"^^xsd:nonNegativeInteger ;
        owl:onClass :ExplanationComponentEvaluation ;
        owl:onProperty gufo:mediates
    ] .

:EvaluationMeasure
    a gufo:Kind, owl:Class, owl:NamedIndividual ;
    rdfs:comment "EvaluationMeasure is a measure to assess the performance of the machine learning model generated by the train operation. Examples are predictive accuracy or f-measure."@en ;
    rdfs:label "EvaluationMeasure"@en ;
    rdfs:subClassOf gufo:FunctionalComplex .

:EvaluationProcedure
    a gufo:SubKind, owl:Class, owl:NamedIndividual ;
    rdfs:comment "EvaluationProcedure is a technique to evaluate machine learning models, being considered specific types of algorithm since they can be implemented in different programming languages. Examples are cross-validation and leave-one-out."@en ;
    rdfs:label "EvaluationProcedure"@en ;
    rdfs:subClassOf :Algorithm .

:EvaluationRIPPERAccuracy
    gufo:isComponentOf :RipperEvaluation ;
    a owl:NamedIndividual, :ExplanationComponentEvaluation .

:EvaluationRipperRule01
    gufo:isComponentOf :RipperEvaluation ;
    a owl:NamedIndividual, :ExplanationComponentEvaluation .

:EvaluationRipperRule02
    gufo:isComponentOf :RipperEvaluation ;
    a owl:NamedIndividual, :ExplanationComponentEvaluation .

:EvaluationRipperRule03
    gufo:isComponentOf :RipperEvaluation ;
    a owl:NamedIndividual, :ExplanationComponentEvaluation .

:EvaluationRipperRule04
    gufo:isComponentOf :RipperEvaluation ;
    a owl:NamedIndividual, :ExplanationComponentEvaluation .

:EvaluationRipperRule05
    gufo:isComponentOf :RipperEvaluation ;
    a owl:NamedIndividual, :ExplanationComponentEvaluation .

:EvaluationRipperRule06
    gufo:isComponentOf :RipperEvaluation ;
    a owl:NamedIndividual, :ExplanationComponentEvaluation .

:EvaluationRipperRule07
    gufo:isComponentOf :RipperEvaluation ;
    a owl:NamedIndividual, :ExplanationComponentEvaluation .

:EvaluationRipperRule08
    gufo:isComponentOf :RipperEvaluation ;
    a owl:NamedIndividual, :ExplanationComponentEvaluation .

:EvaluationRipperRule09
    gufo:isComponentOf :RipperEvaluation ;
    a owl:NamedIndividual, :ExplanationComponentEvaluation .

:EvaluationRipperRule10
    gufo:isComponentOf :RipperEvaluation ;
    a owl:NamedIndividual, :ExplanationComponentEvaluation .

:EvaluationRipperRule11
    gufo:isComponentOf :RipperEvaluation ;
    a owl:NamedIndividual, :ExplanationComponentEvaluation .

:EvaluationRipperRule12
    gufo:isComponentOf :RipperEvaluation ;
    a owl:NamedIndividual, :ExplanationComponentEvaluation .

:EvaluationRipperRule13
    gufo:isComponentOf :RipperEvaluation ;
    a owl:NamedIndividual, :ExplanationComponentEvaluation .

:EvaluationRipperRule14
    gufo:isComponentOf :RipperEvaluation ;
    a owl:NamedIndividual, :ExplanationComponentEvaluation .

:EvaluationRipperRule15
    gufo:isComponentOf :RipperEvaluation ;
    a owl:NamedIndividual, :ExplanationComponentEvaluation .

:EvaluationRipperRule16
    gufo:isComponentOf :RipperEvaluation ;
    a owl:NamedIndividual, :ExplanationComponentEvaluation .

:EvaluationRipperRuleEvaluatesRipperRule01
    a owl:NamedIndividual, :EvaluatesExplanationComponent ;
    :evaluatesInvolvesExplanationComponent :RipperRule01 ;
    :evaluatesInvolvesExplanationComponentEvaluation :EvaluationRipperRule01 .

:EvaluationRipperRuleEvaluatesRipperRule02
    a owl:NamedIndividual, :EvaluatesExplanationComponent ;
    :evaluatesInvolvesExplanationComponent :RipperRule02 ;
    :evaluatesInvolvesExplanationComponentEvaluation :EvaluationRipperRule02 .

:EvaluationRipperRuleEvaluatesRipperRule03
    a owl:NamedIndividual, :EvaluatesExplanationComponent ;
    :evaluatesInvolvesExplanationComponent :RipperRule03 ;
    :evaluatesInvolvesExplanationComponentEvaluation :EvaluationRipperRule03 .

:EvaluationRipperRuleEvaluatesRipperRule04
    a owl:NamedIndividual, :EvaluatesExplanationComponent ;
    :evaluatesInvolvesExplanationComponent :RipperRule04 ;
    :evaluatesInvolvesExplanationComponentEvaluation :EvaluationRipperRule04 .

:EvaluationRipperRuleEvaluatesRipperRule05
    a owl:NamedIndividual, :EvaluatesExplanationComponent ;
    :evaluatesInvolvesExplanationComponent :RipperRule05 ;
    :evaluatesInvolvesExplanationComponentEvaluation :EvaluationRipperRule05 .

:EvaluationRipperRuleEvaluatesRipperRule06
    a owl:NamedIndividual, :EvaluatesExplanationComponent ;
    :evaluatesInvolvesExplanationComponent :RipperRule06 ;
    :evaluatesInvolvesExplanationComponentEvaluation :EvaluationRipperRule06 .

:EvaluationRipperRuleEvaluatesRipperRule07
    a owl:NamedIndividual, :EvaluatesExplanationComponent ;
    :evaluatesInvolvesExplanationComponent :RipperRule07 ;
    :evaluatesInvolvesExplanationComponentEvaluation :EvaluationRipperRule07 .

:EvaluationRipperRuleEvaluatesRipperRule08
    a owl:NamedIndividual, :EvaluatesExplanationComponent ;
    :evaluatesInvolvesExplanationComponent :RipperRule08 ;
    :evaluatesInvolvesExplanationComponentEvaluation :EvaluationRipperRule08 .

:EvaluationRipperRuleEvaluatesRipperRule09
    a owl:NamedIndividual, :EvaluatesExplanationComponent ;
    :evaluatesInvolvesExplanationComponent :RipperRule09 ;
    :evaluatesInvolvesExplanationComponentEvaluation :EvaluationRipperRule09 .

:EvaluationRipperRuleEvaluatesRipperRule10
    a owl:NamedIndividual, :EvaluatesExplanationComponent ;
    :evaluatesInvolvesExplanationComponent :RipperRule10 ;
    :evaluatesInvolvesExplanationComponentEvaluation :EvaluationRipperRule10 .

:EvaluationRipperRuleEvaluatesRipperRule11
    a owl:NamedIndividual, :EvaluatesExplanationComponent ;
    :evaluatesInvolvesExplanationComponent :RipperRule11 ;
    :evaluatesInvolvesExplanationComponentEvaluation :EvaluationRipperRule11 .

:EvaluationRipperRuleEvaluatesRipperRule12
    a owl:NamedIndividual, :EvaluatesExplanationComponent ;
    :evaluatesInvolvesExplanationComponent :RipperRule12 ;
    :evaluatesInvolvesExplanationComponentEvaluation :EvaluationRipperRule12 .

:EvaluationRipperRuleEvaluatesRipperRule13
    a owl:NamedIndividual, :EvaluatesExplanationComponent ;
    :evaluatesInvolvesExplanationComponent :RipperRule13 ;
    :evaluatesInvolvesExplanationComponentEvaluation :EvaluationRipperRule13 .

:EvaluationRipperRuleEvaluatesRipperRule14
    a owl:NamedIndividual, :EvaluatesExplanationComponent ;
    :evaluatesInvolvesExplanationComponent :RipperRule14 ;
    :evaluatesInvolvesExplanationComponentEvaluation :EvaluationRipperRule14 .

:EvaluationRipperRuleEvaluatesRipperRule15
    a owl:NamedIndividual, :EvaluatesExplanationComponent ;
    :evaluatesInvolvesExplanationComponent :RipperRule15 ;
    :evaluatesInvolvesExplanationComponentEvaluation :EvaluationRipperRule15 .

:EvaluationRipperRuleEvaluatesRipperRule16
    a owl:NamedIndividual, :EvaluatesExplanationComponent ;
    :evaluatesInvolvesExplanationComponent :RipperRule16 ;
    :evaluatesInvolvesExplanationComponentEvaluation :EvaluationRipperRule16 .

:EvaluationSPLimeExplanation01
    gufo:isComponentOf :SPLimeEvaluation ;
    a owl:NamedIndividual, :ExplanationComponentEvaluation .

:EvaluationSPLimeExplanation02
    gufo:isComponentOf :SPLimeEvaluation ;
    a owl:NamedIndividual, :ExplanationComponentEvaluation .

:EvaluationSPLimeExplanation03
    gufo:isComponentOf :SPLimeEvaluation ;
    a owl:NamedIndividual, :ExplanationComponentEvaluation .

:EvaluationSPLimeExplanation04
    gufo:isComponentOf :SPLimeEvaluation ;
    a owl:NamedIndividual, :ExplanationComponentEvaluation .

:EvaluationSPLimeExplanation05
    gufo:isComponentOf :SPLimeEvaluation ;
    a owl:NamedIndividual, :ExplanationComponentEvaluation .

:Exp1_field
    gufo:hasQualityValue "Healthcare"^^xsd:string ;
    gufo:inheresIn :Experiment1 ;
    a owl:NamedIndividual, :ExperimentDomain .

:Exp1_type
    gufo:hasQualityValue "Machine Learning and explanation experiment"^^xsd:string ;
    gufo:inheresIn :Experiment1 ;
    a owl:NamedIndividual, :ExperimentType .

:Exp2_field
    gufo:hasQualityValue "Healthcare"^^xsd:string ;
    gufo:inheresIn :Experiment2 ;
    a owl:NamedIndividual, :ExperimentDomain .

:Exp2_type
    gufo:hasQualityValue "ML Experiment"^^xsd:string ;
    gufo:inheresIn :Experiment2 ;
    a owl:NamedIndividual, :ExperimentType .

:Experiment
    a gufo:EventType, owl:Class, owl:NamedIndividual ;
    rdfs:comment "An experiment is a complex process composed of subprocesses that belong together to do some kind of analysis on its results. This analysis can be general or very specific (e.g. a hypothesis test), having a specific goal."@en ;
    rdfs:label "Experiment"@en ;
    rdfs:subClassOf gufo:Event, [
        a owl:Restriction ;
        owl:onProperty gufo:isEventProperPartOf ;
        owl:someValuesFrom :Study
    ], [
        a owl:Restriction ;
        owl:onProperty [
            owl:inverseOf gufo:inheresIn
        ] ;
        owl:someValuesFrom :ExperimentCharacteristic
    ], [
        a owl:Restriction ;
        owl:onProperty [
            owl:inverseOf gufo:isEventProperPartOf
        ] ;
        owl:someValuesFrom :WFExecution
    ], [
        a owl:Restriction ;
        owl:minQualifiedCardinality "1"^^xsd:nonNegativeInteger ;
        owl:onClass :Goal ;
        owl:onProperty [
            owl:inverseOf gufo:participatedIn
        ]
    ] .

:Experiment1
    dc:creator "Patricia"@en ;
    gufo:hasBeginPointInXSDDate "26-05-2021"^^xsd:date ;
    gufo:hasEndPointInXSDDate "26-05-2021"^^xsd:date ;
    a owl:NamedIndividual, :Experiment ;
    rdfs:comment "Predict mortality of confirmed cases using Epidemiology dataset of tested people for COVID-19 in Mexico and generate explanation using RIPPER."@en .

:Experiment2
    dc:creator "Patricia"@en ;
    gufo:hasBeginPointInXSDDate "31-05-2021"^^xsd:date ;
    gufo:hasEndPointInXSDDate "31-05-2021"^^xsd:date ;
    a owl:NamedIndividual, :Experiment ;
    rdfs:comment "Predict mortality of confirmed cases using Epidemiology dataset of tested people for COVID-19 in Mexico and generate explanation using LIME."@en .

:ExperimentCharacteristic
    a gufo:Kind, owl:Class, owl:NamedIndividual ;
    rdfs:comment "Characteristics of the Experiment."@en ;
    rdfs:label "ExperimentCharacteristic"@en ;
    rdfs:subClassOf gufo:Quality, [
        a owl:Restriction ;
        owl:minQualifiedCardinality "1"^^xsd:nonNegativeInteger ;
        owl:onClass :Experiment ;
        owl:onProperty gufo:inheresIn
    ] .

:ExperimentDomain
    a gufo:SubKind, owl:Class, owl:NamedIndividual ;
    rdfs:comment "Indicates the domain of the experiment, for example, healthcare."@en ;
    rdfs:label "ExperimentDomain"@en ;
    rdfs:subClassOf :ExperimentCharacteristic .

:ExperimentType
    a gufo:SubKind, owl:Class, owl:NamedIndividual ;
    rdfs:comment "Indicates the type of experiment, for example, a machine learning experiment."@en ;
    rdfs:label "ExperimentType"@en ;
    rdfs:subClassOf :ExperimentCharacteristic .

:Explain
    a gufo:EventType, owl:Class, owl:NamedIndividual ;
    rdfs:comment "Specific type of operation that focus on generating the explanations from the MLModel."@en ;
    rdfs:label "Explain"@en ;
    rdfs:subClassOf :Operation, [
        a owl:Restriction ;
        owl:minQualifiedCardinality "1"^^xsd:nonNegativeInteger ;
        owl:onClass :ExplainImplementation ;
        owl:onProperty [
            owl:inverseOf gufo:participatedIn
        ]
    ], [
        a owl:Restriction ;
        owl:onClass :Train ;
        owl:onProperty gufo:historicallyDependsOn ;
        owl:qualifiedCardinality "1"^^xsd:nonNegativeInteger
    ], [
        a owl:Restriction ;
        owl:onClass :Explanation ;
        owl:onProperty [
            owl:inverseOf gufo:wasCreatedIn
        ] ;
        owl:qualifiedCardinality "1"^^xsd:nonNegativeInteger
    ] .

:ExplainImplementation
    a gufo:SubKind, owl:Class, owl:NamedIndividual ;
    rdfs:comment "Specific type of implementation that implements the explainable algorithm."@en ;
    rdfs:label "ExplainImplementation"@en ;
    rdfs:subClassOf :Implementation .

:ExplainSVMLIME
    gufo:historicallyDependsOn :TrainSVM ;
    gufo:isEventProperPartOf :ExplainWorkflow_exec_exp2 ;
    a owl:NamedIndividual, :Explain .

:ExplainSVMRIPPER
    dc:creator "Patricia"^^xsd:string ;
    gufo:historicallyDependsOn :TrainSVM ;
    gufo:isEventProperPartOf :ExplainWorkflow_exec_exp1 ;
    a owl:NamedIndividual, :Explain ;
    rdfs:comment "Generate explanations of the ML model using the RIPPER method to extract rules."^^xsd:string .

:ExplainWorfklow_exp2
    gufo:participatedIn :ExplainWorkflow_exec_exp2 ;
    a owl:NamedIndividual, :Workflow .

:ExplainWorkflow_exec_exp1
    dc:creator "Patricia"^^xsd:string ;
    gufo:hasBeginPointInXSDDate "26-05-2021"^^xsd:date ;
    gufo:hasEndPointInXSDDate "26-05-2021"^^xsd:date ;
    gufo:isEventProperPartOf :Experiment1 ;
    a owl:NamedIndividual, :WFExecution ;
    rdfs:comment "Workflow to generate and evaluate explanations from the ML Model."^^xsd:string .

:ExplainWorkflow_exec_exp2
    dc:creator "Patricia"@en ;
    gufo:hasBeginPointInXSDDate "31-05-2021"^^xsd:date ;
    gufo:hasEndPointInXSDDate "31-05-2021"^^xsd:date ;
    gufo:isEventProperPartOf :Experiment2 ;
    a owl:NamedIndividual, :WFExecution ;
    rdfs:comment "Workflow to generate and evaluate explanations from the ML Model."@en .

:ExplainWorkflow_exp1
    dc:creator "Patricia"^^xsd:string ;
    gufo:participatedIn :ExplainWorkflow_exec_exp1 ;
    a owl:NamedIndividual, :Workflow ;
    rdfs:comment "Workflow that contains the implementation steps of the explanation process, executed by WFExecution."^^xsd:string .

:ExplainableAlgorithm
    a gufo:SubKind, owl:Class, owl:NamedIndividual ;
    rdfs:comment "Specific type of post-hoc methods that focus on generating explanations from the MLModel."@en ;
    rdfs:label "ExplainableAlgorithm"@en ;
    rdfs:subClassOf :Algorithm .

:ExplainableMethodFlexibility
    a owl:Class ;
    rdfs:comment "ExplainableMethodFlexibility"@en, "Identifies if the post-hoc method is model-specific or model-agnostic."@en ;
    rdfs:subClassOf gufo:QualityValue .

:ExplainedElement
    a gufo:AbstractIndividualType, owl:Class, owl:NamedIndividual ;
    rdfs:comment "Element that is explained by the explanation, i.e., if it explains the logic behind the ML Model or the result."@en ;
    rdfs:label "ExplainedElement"@en ;
    rdfs:subClassOf gufo:QualityValue .

:ExplainedElementMLModel
    a owl:NamedIndividual, :ExplainedElement ;
    rdfs:comment "Indicates that the explainable method generates explanations that explains the logic behind the ML model." .

:ExplainedElementOutput
    a owl:NamedIndividual, :ExplainedElement ;
    rdfs:comment "Indicates that the explainable method generates explanations that explains one output instance." .

:ExplainsModel
    a gufo:Kind, owl:Class, owl:NamedIndividual ;
    rdfs:comment "Relator that indicates that the Model Explanation explains the ML Model. It enables retrieving the logic behind the ML Model after the post-hoc method is applied."@en ;
    rdfs:label "ExplainsModel"@en ;
    rdfs:subClassOf gufo:Relator, [
        a owl:Restriction ;
        owl:minQualifiedCardinality "1"^^xsd:nonNegativeInteger ;
        owl:onClass :MLModel ;
        owl:onProperty gufo:mediates
    ], [
        a owl:Restriction ;
        owl:minQualifiedCardinality "1"^^xsd:nonNegativeInteger ;
        owl:onClass :ModelExplanation ;
        owl:onProperty gufo:mediates
    ] .

:ExplainsResultInstance
    a gufo:Kind, owl:Class, owl:NamedIndividual ;
    rdfs:comment "Relator that indicates that the explanation component explains the result instance, enabling retrieving the explanation of a specific instance of the result."@en ;
    rdfs:label "ExplainsResultInstance"@en ;
    rdfs:subClassOf gufo:Relator, [
        a owl:Restriction ;
        owl:minQualifiedCardinality "1"^^xsd:nonNegativeInteger ;
        owl:onClass :ExplanationComponent ;
        owl:onProperty gufo:mediates
    ], [
        a owl:Restriction ;
        owl:minQualifiedCardinality "1"^^xsd:nonNegativeInteger ;
        owl:onClass :ResultInstance ;
        owl:onProperty gufo:mediates
    ] .

:Explanation
    a gufo:Kind, owl:Class, owl:NamedIndividual ;
    rdfs:comment "Type of output that is generated by the explain operation, which contains the explanation generated by the post-hoc method."@en ;
    rdfs:label "Explanation"@en ;
    rdfs:subClassOf :Output, [
        a owl:Restriction ;
        owl:onClass :Explain ;
        owl:onProperty gufo:wasCreatedIn ;
        owl:qualifiedCardinality "1"^^xsd:nonNegativeInteger
    ] .

:ExplanationAccuracy
    a gufo:SubKind, owl:Class, owl:NamedIndividual ;
    rdfs:comment "Accuracy is the proportion of correct predictions (both true positives and true negatives) among the total number of cases examined."^^xsd:string ;
    rdfs:label "ExplanationAccuracy"@en ;
    rdfs:subClassOf :ExplanationComponentEvaluationCharacteristic .

:ExplanationComponent
    a gufo:Kind, owl:Class, owl:NamedIndividual ;
    rdfs:comment "Components of the Explanation, which can represent explanation of a single instance or one single rule."@en ;
    rdfs:label "ExplanationComponent"@en ;
    rdfs:subClassOf gufo:FunctionalComplex, [
        a owl:Restriction ;
        owl:onProperty [
            owl:inverseOf gufo:mediates
        ] ;
        owl:someValuesFrom :ExplainsResultInstance
    ], [
        a owl:Restriction ;
        owl:onClass :Explanation ;
        owl:onProperty gufo:isComponentOf ;
        owl:qualifiedCardinality "1"^^xsd:nonNegativeInteger
    ] .

:ExplanationComponentCharacteristic
    a gufo:Kind, owl:Class, owl:NamedIndividual ;
    rdfs:comment "Characteristics of the Explanation Component."@en ;
    rdfs:label "ExplanationComponentCharacteristic"@en ;
    rdfs:subClassOf gufo:Quality, [
        a owl:Restriction ;
        owl:onClass :ExplanationComponent ;
        owl:onProperty gufo:inheresIn ;
        owl:qualifiedCardinality "1"^^xsd:nonNegativeInteger
    ] .

:ExplanationComponentEvaluation
    a gufo:Kind, owl:Class, owl:NamedIndividual ;
    rdfs:comment "A component of the explanation evaluation that evaluates explanation components (e.g., coverage), instead of evaluating the whole explanations (in the case of trustworthiness)."@en ;
    rdfs:label "ExplanationComponentEvaluation"@en ;
    rdfs:subClassOf gufo:FunctionalComplex, [
        a owl:Restriction ;
        owl:onProperty [
            owl:inverseOf gufo:mediates
        ] ;
        owl:someValuesFrom :EvaluatesExplanationComponent
    ], [
        a owl:Restriction ;
        owl:onClass :ExplanationEvaluation ;
        owl:onProperty gufo:isComponentOf ;
        owl:qualifiedCardinality "1"^^xsd:nonNegativeInteger
    ] .

:ExplanationComponentEvaluationCharacteristic
    a gufo:Kind, owl:Class, owl:NamedIndividual ;
    rdfs:comment "Characteristics of the Explanation Component Evaluation."@en ;
    rdfs:label "ExplanationComponentEvaluationCharacteristic"@en ;
    rdfs:subClassOf gufo:Quality, [
        a owl:Restriction ;
        owl:minQualifiedCardinality "1"^^xsd:nonNegativeInteger ;
        owl:onClass :ExplanationComponentEvaluation ;
        owl:onProperty gufo:inheresIn
    ] .

:ExplanationCoverage
    a gufo:SubKind, owl:Class, owl:NamedIndividual ;
    rdfs:comment "Number of instances covered by the Explanation Component."@en ;
    rdfs:label "ExplanationCoverage"@en ;
    rdfs:subClassOf :ExplanationComponentEvaluationCharacteristic .

:ExplanationEvaluation
    a gufo:Kind, owl:Class, owl:NamedIndividual ;
    rdfs:comment "Type of output that is generated by the evaluate explanation operation. It can indicate, for example, the trustworthiness of the Explanation or the coverage of its components."@en ;
    rdfs:label "ExplanationEvaluation"@en ;
    rdfs:subClassOf :Output, [
        a owl:Restriction ;
        owl:onClass :EvaluateExplanation ;
        owl:onProperty gufo:wasCreatedIn ;
        owl:qualifiedCardinality "1"^^xsd:nonNegativeInteger
    ] .

:ExplanationEvaluationCharacteristic
    a gufo:Kind, owl:NamedIndividual .

:ExplanationFidelity
    a owl:Class ;
    rdfs:comment "Indicates how faithful the explanation is to the underlying ML model."@en ;
    rdfs:label "ExplanationFidelity"@en ;
    rdfs:subClassOf gufo:QualityValue .

:ExplanationFormat
    a gufo:AbstractIndividualType, owl:Class, owl:NamedIndividual ;
    rdfs:comment "Type of explanation generated by the algorithm"@en ;
    rdfs:label "ExplanationFormat"@en ;
    rdfs:subClassOf gufo:QualityValue .

:ExplanationInteraction
    a gufo:AbstractIndividualType, owl:Class, owl:NamedIndividual ;
    rdfs:comment "Indicates if the explanation generated by the algorithm is static or interactive."@en ;
    rdfs:label "ExplanationInteraction"@en ;
    rdfs:subClassOf gufo:QualityValue .

:ExplanationScope
    a gufo:AbstractIndividualType, owl:Class, owl:NamedIndividual ;
    rdfs:comment "Scope of the explainable algorithm."@en ;
    rdfs:label "ExplanationScope"@en ;
    rdfs:subClassOf gufo:QualityValue .

:Feature
    a gufo:Kind, owl:Class, owl:NamedIndividual ;
    rdfs:comment "Features are measurable properties or characteristic of a phenomenon. In a dataset, they can be the input variables."@en ;
    rdfs:label "Feature"@en ;
    rdfs:subClassOf gufo:FunctionalComplex, [
        a owl:Restriction ;
        owl:onProperty [
            owl:inverseOf gufo:inheresIn
        ] ;
        owl:someValuesFrom :FeatureCharacteristic
    ], [
        a owl:Restriction ;
        owl:onClass :Data ;
        owl:onProperty gufo:isComponentOf ;
        owl:qualifiedCardinality "1"^^xsd:nonNegativeInteger
    ] .

:FeatureCharacteristic
    a gufo:Kind, owl:Class, owl:NamedIndividual ;
    rdfs:comment "Characteristics of the features."@en ;
    rdfs:label "FeatureCharacteristic"@en ;
    rdfs:subClassOf gufo:Quality, [
        a owl:Restriction ;
        owl:minQualifiedCardinality "1"^^xsd:nonNegativeInteger ;
        owl:onClass :Feature ;
        owl:onProperty gufo:inheresIn
    ] .

:FeatureExtraction
    a owl:NamedIndividual, :PreprocessingTechnique ;
    rdfs:comment "Indicates that the preprocessing technique is related to extracting features of the data." .

:Global
    a owl:NamedIndividual, :ExplanationScope ;
    rdfs:comment "Indicates that the scope of the explainable method is global, that is, considers the whole dataset." .

:Goal
    a gufo:Kind, owl:Class, owl:NamedIndividual ;
    rdfs:comment "The main goal of the study, for example, diagnosis of patients with Covid-19."@en ;
    rdfs:label "Goal"@en ;
    rdfs:subClassOf gufo:FunctionalComplex, [
        a owl:Restriction ;
        owl:onProperty gufo:participatedIn ;
        owl:someValuesFrom :Experiment
    ] .

:GoalCharacteristic
    a gufo:Kind, owl:Class, owl:NamedIndividual ;
    rdfs:comment "Characteristics of the goal of the experiment."@en ;
    rdfs:label "GoalCharacteristic"@en ;
    rdfs:subClassOf gufo:Quality, [
        a owl:Restriction ;
        owl:onProperty gufo:inheresIn ;
        owl:someValuesFrom :Goal
    ] .

:GoalSpecifiesAccuracy_exp1
    a owl:NamedIndividual, :SpecifiesMeasure ;
    :specifiesMeasureInvolvesGoal :ClassifyMortality_exp1 ;
    :specifiesMeasureInvolvesMeasure :Accuracy .

:GoalSpecifiesAccuracy_exp2
    a owl:NamedIndividual, :SpecifiesMeasure ;
    :specifiesMeasureInvolvesGoal :ClassifyMortality_exp2 ;
    :specifiesMeasureInvolvesMeasure :Accuracy .

:GoalSpecifiesSensitivity_exp1
    a owl:NamedIndividual, :SpecifiesMeasure ;
    :specifiesMeasureInvolvesGoal :ClassifyMortality_exp1 ;
    :specifiesMeasureInvolvesMeasure :Sensitivity .

:GoalSpecifiesSensitivity_exp2
    a owl:NamedIndividual, :SpecifiesMeasure ;
    :specifiesMeasureInvolvesGoal :ClassifyMortality_exp2 ;
    :specifiesMeasureInvolvesMeasure :Sensitivity .

:GoalSpecifiesSpecificity_exp1
    a owl:NamedIndividual, :SpecifiesMeasure ;
    :specifiesMeasureInvolvesGoal :ClassifyMortality_exp1 ;
    :specifiesMeasureInvolvesMeasure :Specificity .

:GoalSpecifiesSpecificity_exp2
    a owl:NamedIndividual, :SpecifiesMeasure ;
    :specifiesMeasureInvolvesGoal :ClassifyMortality_exp2 ;
    :specifiesMeasureInvolvesMeasure :Specificity .

:HasMeasure
    a gufo:Kind, owl:Class, owl:NamedIndividual ;
    rdfs:comment "Relator that indicates that implementation of the evaluation procedure takes into account the evaluation measurements."@en ;
    rdfs:label "HasMeasure"@en ;
    rdfs:subClassOf gufo:Relator, [
        a owl:Restriction ;
        owl:minQualifiedCardinality "1"^^xsd:nonNegativeInteger ;
        owl:onClass :EvaluateModelImplementation ;
        owl:onProperty gufo:mediates
    ], [
        a owl:Restriction ;
        owl:minQualifiedCardinality "1"^^xsd:nonNegativeInteger ;
        owl:onClass :EvaluationMeasure ;
        owl:onProperty gufo:mediates
    ] .

:HasParameter
    a gufo:Kind, owl:Class, owl:NamedIndividual ;
    rdfs:comment "Relator that indicates that the Implementation may have Parameter(s)."@en ;
    rdfs:label "HasParameter"@en ;
    rdfs:subClassOf gufo:Relator, [
        a owl:Restriction ;
        owl:minQualifiedCardinality "1"^^xsd:nonNegativeInteger ;
        owl:onClass :Implementation ;
        owl:onProperty gufo:mediates
    ], [
        a owl:Restriction ;
        owl:minQualifiedCardinality "1"^^xsd:nonNegativeInteger ;
        owl:onClass :Parameter ;
        owl:onProperty gufo:mediates
    ] .

:HospitalizedCorrelatesAge
    a owl:NamedIndividual, :Correlates ;
    :correlates :Age_Covid-19Train, :PatientType_Covid-19Train .

:HospitalizedCorrelatesAgeValue
    gufo:hasQualityValue 0.402038 ;
    gufo:inheresIn :HospitalizedCorrelatesAge ;
    a owl:NamedIndividual, :CorrelationCharacteristic .

:Hospitalized_Covid-19Train_1
    gufo:hasQualityValue 4843 ;
    gufo:inheresIn :PatientType_Covid-19Train ;
    a owl:NamedIndividual, :CategoryQuantity .

:Hospitalized_Covid-19Train_2
    gufo:hasQualityValue 1772 ;
    gufo:inheresIn :PatientType_Covid-19Train ;
    a owl:NamedIndividual, :CategoryQuantity .

:HypertensionCorrelatesDiabetes
    a owl:NamedIndividual, :Correlates ;
    :correlates :Diabetes_Covid-19Train, :Hypertension_Covid-19Train .

:HypertensionCorrelatesDiabetesValue
    gufo:hasQualityValue 0.364664 ;
    gufo:inheresIn :HypertensionCorrelatesDiabetes ;
    a owl:NamedIndividual, :CorrelationCharacteristic .

:HypertensionCorrelatesICU
    a owl:NamedIndividual, :Correlates ;
    :correlates :Hypertension_Covid-19Train, :ICU_Covid-19Train .

:HypertensionCorrelatesICUValue
    gufo:hasQualityValue 0.252025 ;
    gufo:inheresIn :HypertensionCorrelatesICU ;
    a owl:NamedIndividual, :CorrelationCharacteristic .

:HypertensionCorrelatesPneumonia
    a owl:NamedIndividual, :Correlates ;
    :correlates :Hypertension_Covid-19Train, :Pneumonia_Covid-19Train .

:HypertensionCorrelatesPneumoniaValue
    gufo:hasQualityValue 0.210804 ;
    gufo:inheresIn :HypertensionCorrelatesPneumonia ;
    a owl:NamedIndividual, :CorrelationCharacteristic .

:Hypertension_Covid-19
    gufo:hasReifiedQualityValue :Categorical ;
    gufo:isComponentOf :Covid-19 ;
    a owl:NamedIndividual, :Feature ;
    rdfs:comment "HYPERTENSION Identifies if the patient has a diagnosis of hypertension."@en .

:Hypertension_Covid-19Test
    gufo:hasReifiedQualityValue :Categorical ;
    gufo:isComponentOf :Covid-19TestData ;
    a owl:NamedIndividual, :Feature ;
    rdfs:comment "HYPERTENSION Identifies if the patient has a diagnosis of hypertension."@en .

:Hypertension_Covid-19Test_categories
    gufo:hasQualityValue "1 = Yes , 2 = No"^^xsd:string ;
    gufo:inheresIn :Hypertension_Covid-19Test ;
    a owl:NamedIndividual, :Categories .

:Hypertension_Covid-19Train
    gufo:hasReifiedQualityValue :Categorical ;
    gufo:isComponentOf :Covid-19TrainData ;
    a owl:NamedIndividual, :Feature ;
    rdfs:comment "HYPERTENSION Identifies if the patient has a diagnosis of hypertension."@en .

:Hypertension_Covid-19Train_1
    gufo:hasQualityValue 1259 ;
    gufo:inheresIn :Hypertension_Covid-19Train ;
    a owl:NamedIndividual, :CategoryQuantity .

:Hypertension_Covid-19Train_2
    gufo:hasQualityValue 5356 ;
    gufo:inheresIn :Hypertension_Covid-19Train ;
    a owl:NamedIndividual, :CategoryQuantity .

:Hypertension_Covid-19Train_categories
    gufo:hasQualityValue "1 = Yes , 2 = No"^^xsd:string ;
    gufo:inheresIn :Hypertension_Covid-19Train ;
    a owl:NamedIndividual, :Categories .

:Hypertension_Covid-19_1
    gufo:hasQualityValue 92508 ;
    gufo:inheresIn :Hypertension_Covid-19 ;
    a owl:NamedIndividual, :CategoryQuantity .

:Hypertension_Covid-19_2
    gufo:hasQualityValue 472270 ;
    gufo:inheresIn :Hypertension_Covid-19 ;
    a owl:NamedIndividual, :CategoryQuantity .

:Hypertension_Covid-19_Null
    gufo:hasQualityValue 1824 ;
    gufo:inheresIn :Hypertension_Covid-19 ;
    a owl:NamedIndividual, :NumberNulls .

:Hypertension_Covid-19_categories
    gufo:hasQualityValue "1 = Yes , 2 = No"^^xsd:string ;
    gufo:inheresIn :Hypertension_Covid-19 ;
    a owl:NamedIndividual, :Categories .

:ICU_Covid-19
    gufo:hasReifiedQualityValue :Categorical ;
    gufo:isComponentOf :Covid-19 ;
    a owl:NamedIndividual, :Feature ;
    rdfs:comment "ICU Identifies if the patient required to enter an Intensive Care Unit."@en .

:ICU_Covid-19Test
    gufo:hasReifiedQualityValue :Categorical ;
    gufo:isComponentOf :Covid-19TestData ;
    a owl:NamedIndividual, :Feature ;
    rdfs:comment "ICU Identifies if the patient required to enter an Intensive Care Unit."@en .

:ICU_Covid-19Test_categories
    gufo:hasQualityValue "1 = Yes, 2 = No, 97 = Not applicable"^^xsd:string ;
    gufo:inheresIn :ICU_Covid-19Test ;
    a owl:NamedIndividual, :Categories .

:ICU_Covid-19Train
    gufo:hasReifiedQualityValue :Categorical ;
    gufo:isComponentOf :Covid-19TrainData ;
    a owl:NamedIndividual, :Feature ;
    rdfs:comment "ICU Identifies if the patient required to enter an Intensive Care Unit."@en .

:ICU_Covid-19Train_1
    gufo:hasQualityValue 136 ;
    gufo:inheresIn :ICU_Covid-19Train ;
    a owl:NamedIndividual, :CategoryQuantity .

:ICU_Covid-19Train_2
    gufo:hasQualityValue 1636 ;
    gufo:inheresIn :ICU_Covid-19Train ;
    a owl:NamedIndividual, :CategoryQuantity .

:ICU_Covid-19Train_97
    gufo:hasQualityValue 4843 ;
    gufo:inheresIn :ICU_Covid-19Train ;
    a owl:NamedIndividual, :CategoryQuantity .

:ICU_Covid-19Train_categories
    gufo:hasQualityValue "1 = Yes, 2 = No, 97 = Not applicable"^^xsd:string ;
    gufo:inheresIn :ICU_Covid-19Train ;
    a owl:NamedIndividual, :Categories .

:ICU_Covid-19_1
    gufo:hasQualityValue 10112 ;
    gufo:inheresIn :ICU_Covid-19 ;
    a owl:NamedIndividual, :CategoryQuantity .

:ICU_Covid-19_2
    gufo:hasQualityValue 111676 ;
    gufo:inheresIn :ICU_Covid-19 ;
    a owl:NamedIndividual, :CategoryQuantity .

:ICU_Covid-19_97
    gufo:hasQualityValue 444689 ;
    gufo:inheresIn :ICU_Covid-19 ;
    a owl:NamedIndividual, :CategoryQuantity .

:ICU_Covid-19_Null
    gufo:hasQualityValue 125 ;
    gufo:inheresIn :ICU_Covid-19 ;
    a owl:NamedIndividual, :NumberNulls .

:ICU_Covid-19_categories
    gufo:hasQualityValue "1 = Yes, 2 = No, 97 = Not applicable"^^xsd:string ;
    gufo:inheresIn :ICU_Covid-19 ;
    a owl:NamedIndividual, :Categories .

:ID_Covid-19
    gufo:hasReifiedQualityValue :Discrete ;
    gufo:isComponentOf :Covid-19 ;
    a owl:NamedIndividual, :Feature ;
    rdfs:comment "Case identifier number"@en .

:Image
    a owl:NamedIndividual, :DataType .

:ImageHighlight
    a owl:NamedIndividual, :ExplanationFormat ;
    rdfs:comment "Indicates that the explainable method generates explanations in the format of highlighted pixels in a image." .

:Immunosuppression_Covid-19
    gufo:hasReifiedQualityValue :Categorical ;
    gufo:isComponentOf :Covid-19 ;
    a owl:NamedIndividual, :Feature ;
    rdfs:comment "Identifies if the patient has immunosuppression."@en .

:Immunosuppression_Covid-19Test
    gufo:hasReifiedQualityValue :Categorical ;
    gufo:isComponentOf :Covid-19TestData ;
    a owl:NamedIndividual, :Feature ;
    rdfs:comment "Identifies if the patient has immunosuppression."@en .

:Immunosuppression_Covid-19Test_categories
    gufo:hasQualityValue "1 = Yes , 2 = No"^^xsd:string ;
    gufo:inheresIn :Immunosuppression_Covid-19Test ;
    a owl:NamedIndividual, :Categories .

:Immunosuppression_Covid-19Train
    gufo:hasReifiedQualityValue :Categorical ;
    gufo:isComponentOf :Covid-19TrainData ;
    a owl:NamedIndividual, :Feature ;
    rdfs:comment "Identifies if the patient has immunosuppression."@en .

:Immunosuppression_Covid-19Train_1
    gufo:hasQualityValue 88 ;
    gufo:inheresIn :Immunosuppression_Covid-19Train ;
    a owl:NamedIndividual, :CategoryQuantity .

:Immunosuppression_Covid-19Train_2
    gufo:hasQualityValue 6527 ;
    gufo:inheresIn :Immunosuppression_Covid-19Train ;
    a owl:NamedIndividual, :CategoryQuantity .

:Immunosuppression_Covid-19Train_categories
    gufo:hasQualityValue "1 = Yes , 2 = No"^^xsd:string ;
    gufo:inheresIn :Immunosuppression_Covid-19Train ;
    a owl:NamedIndividual, :Categories .

:Immunosuppression_Covid-19_1
    gufo:hasQualityValue 8978 ;
    gufo:inheresIn :Immunosuppression_Covid-19 ;
    a owl:NamedIndividual, :CategoryQuantity .

:Immunosuppression_Covid-19_2
    gufo:hasQualityValue 555644 ;
    gufo:inheresIn :Immunosuppression_Covid-19 ;
    a owl:NamedIndividual, :CategoryQuantity .

:Immunosuppression_Covid-19_Null
    gufo:hasQualityValue 1980 ;
    gufo:inheresIn :Immunosuppression_Covid-19 ;
    a owl:NamedIndividual, :NumberNulls .

:Immunosuppression_Covid-19_categories
    gufo:hasQualityValue "1 = Yes, 2 = No"^^xsd:string ;
    gufo:inheresIn :Immunosuppression_Covid-19 ;
    a owl:NamedIndividual, :Categories .

:Implementation
    a gufo:Kind, owl:Class, owl:NamedIndividual ;
    rdfs:comment " Implementation is an executable implementation of an algorithm. It is versioned, and sometimes belongs to a library (e.g. WEKA)."@en ;
    rdfs:label "Implementation"@en ;
    rdfs:subClassOf gufo:FunctionalComplex, [
        a owl:Restriction ;
        owl:onProperty gufo:isComponentOf ;
        owl:someValuesFrom :Workflow
    ], [
        a owl:Restriction ;
        owl:onProperty [
            owl:inverseOf gufo:inheresIn
        ] ;
        owl:someValuesFrom :ImplementationCharacteristic
    ], [
        a owl:Restriction ;
        owl:onClass :Software ;
        owl:onProperty gufo:isComponentOf ;
        owl:qualifiedCardinality "1"^^xsd:nonNegativeInteger
    ] .

:ImplementationCharacteristic
    a gufo:Kind, owl:Class, owl:NamedIndividual ;
    rdfs:comment "Characteristics of the implementation."@en ;
    rdfs:label "ImplementationCharacteristic"@en ;
    rdfs:subClassOf gufo:Quality, [
        a owl:Restriction ;
        owl:minQualifiedCardinality "1"^^xsd:nonNegativeInteger ;
        owl:onClass :Implementation ;
        owl:onProperty gufo:inheresIn
    ] .

:ImplementationLibrary
    a gufo:SubKind, owl:Class, owl:NamedIndividual ;
    rdfs:comment "Indicates the library if the implementation is implemented by a package or library."@en ;
    rdfs:label "ImplementationLibrary"@en ;
    rdfs:subClassOf :ImplementationCharacteristic .

:Implements
    a gufo:Kind, owl:Class, owl:NamedIndividual ;
    rdfs:comment "Relator that indicates that the Implementation implements an Algorithm."@en ;
    rdfs:label "Implements"@en ;
    rdfs:subClassOf gufo:Relator, [
        a owl:Restriction ;
        owl:minQualifiedCardinality "1"^^xsd:nonNegativeInteger ;
        owl:onClass :Algorithm ;
        owl:onProperty gufo:mediates
    ], [
        a owl:Restriction ;
        owl:minQualifiedCardinality "1"^^xsd:nonNegativeInteger ;
        owl:onClass :Implementation ;
        owl:onProperty gufo:mediates
    ] .

:InputData
    a gufo:Phase, owl:Class, owl:NamedIndividual ;
    rdfs:comment "Input data is the data used in the experiment. It is a phase of the data, representing the raw data prior to the preprocessing step."@en ;
    rdfs:label "InputData"@en ;
    rdfs:subClassOf :Data ;
    owl:disjointWith :PreprocessedData .

:InputVariableWeight
    a owl:NamedIndividual, :ExplanationFormat ;
    rdfs:comment "Indicates that the explainable method generates explanations in the format of variable weights in a text or tabular data." .

:Inscrutable
    a owl:NamedIndividual, :Interpretability ;
    rdfs:comment "Indicates that the ML algorithm is inscrutable (not trasparent)." .

:Interactive
    a owl:NamedIndividual, :ExplanationInteraction ;
    rdfs:comment "Indicates that the explainable method generates explanations that are interactive." .

:Interpretability
    a gufo:AbstractIndividualType, owl:Class, owl:NamedIndividual ;
    rdfs:label "MLInterpretability"@en ;
    rdfs:subClassOf gufo:QualityValue .

:IntubedCorrelatesDiabetes
    a owl:NamedIndividual, :Correlates ;
    :correlates :Diabetes_Covid-19Train, :Intubed_Covid-19Train .

:IntubedCorrelatesDiabetesValue
    gufo:hasQualityValue 0.245839 ;
    gufo:inheresIn :IntubedCorrelatesDiabetes ;
    a owl:NamedIndividual, :CorrelationCharacteristic .

:IntubedCorrelatesHypertension
    a owl:NamedIndividual, :Correlates ;
    :correlates :Hypertension_Covid-19Train, :Intubed_Covid-19Train .

:IntubedCorrelatesHypertensionValue
    gufo:hasQualityValue 0.253902 ;
    gufo:inheresIn :IntubedCorrelatesHypertension ;
    a owl:NamedIndividual, :CorrelationCharacteristic .

:IntubedCorrelatesICU
    a owl:NamedIndividual, :Correlates ;
    :correlates :ICU_Covid-19Train, :Intubed_Covid-19Train .

:IntubedCorrelatesICUValue
    gufo:hasQualityValue 0.995625 ;
    gufo:inheresIn :IntubedCorrelatesICU ;
    a owl:NamedIndividual, :CorrelationCharacteristic .

:IntubedCorrelatesPneumonia
    a owl:NamedIndividual, :Correlates ;
    :correlates :Intubed_Covid-19Train, :Pneumonia_Covid-19Train .

:IntubedCorrelatesPneumoniaValue
    gufo:hasQualityValue 0.658587 ;
    gufo:inheresIn :IntubedCorrelatesPneumonia ;
    a owl:NamedIndividual, :CorrelationCharacteristic .

:Intubed_Covid-19
    gufo:hasReifiedQualityValue :Categorical ;
    gufo:isComponentOf :Covid-19 ;
    a owl:NamedIndividual, :Feature ;
    rdfs:comment "Identifies if the patient required intubation."@en .

:Intubed_Covid-19Test
    gufo:hasReifiedQualityValue :Categorical ;
    gufo:isComponentOf :Covid-19TestData ;
    a owl:NamedIndividual, :Feature ;
    rdfs:comment "Identifies if the patient required intubation."@en .

:Intubed_Covid-19Test_categories
    gufo:hasQualityValue "1 = Yes, 2 = No, 97 = Not applicable"^^xsd:string ;
    gufo:inheresIn :Intubed_Covid-19Test ;
    a owl:NamedIndividual, :Categories .

:Intubed_Covid-19Train
    gufo:hasReifiedQualityValue :Categorical ;
    gufo:isComponentOf :Covid-19TrainData ;
    a owl:NamedIndividual, :Feature ;
    rdfs:comment "Identifies if the patient required intubation."@en .

:Intubed_Covid-19Train_1
    gufo:hasQualityValue 143 ;
    gufo:inheresIn :Intubed_Covid-19Train ;
    a owl:NamedIndividual, :CategoryQuantity .

:Intubed_Covid-19Train_2
    gufo:hasQualityValue 1629 ;
    gufo:inheresIn :Intubed_Covid-19Train ;
    a owl:NamedIndividual, :CategoryQuantity .

:Intubed_Covid-19Train_97
    gufo:hasQualityValue 4843 ;
    gufo:inheresIn :Intubed_Covid-19Train ;
    a owl:NamedIndividual, :CategoryQuantity .

:Intubed_Covid-19Train_categories
    gufo:hasQualityValue "1 = Yes, 2 = No, 97 = Not applicable"^^xsd:string ;
    gufo:inheresIn :Intubed_Covid-19Train ;
    a owl:NamedIndividual, :Categories .

:Intubed_Covid-19_1
    gufo:hasQualityValue 9965 ;
    gufo:inheresIn :Intubed_Covid-19 ;
    a owl:NamedIndividual, :CategoryQuantity .

:Intubed_Covid-19_2
    gufo:hasQualityValue 111824 ;
    gufo:inheresIn :Intubed_Covid-19 ;
    a owl:NamedIndividual, :CategoryQuantity .

:Intubed_Covid-19_97
    gufo:hasQualityValue 444689 ;
    gufo:inheresIn :Intubed_Covid-19 ;
    a owl:NamedIndividual, :CategoryQuantity .

:Intubed_Covid-19_Null
    gufo:hasQualityValue 124 ;
    gufo:inheresIn :Intubed_Covid-19 ;
    a owl:NamedIndividual, :NumberNulls .

:Intubed_Covid-19_categories
    gufo:hasQualityValue "1 = Yes, 2 = No, 97 = Not applicable"^^xsd:string ;
    gufo:inheresIn :Intubed_Covid-19 ;
    a owl:NamedIndividual, :Categories .

:KernelSpecifiesKernelType
    a owl:NamedIndividual, :SpecifiesParameter ;
    :specifiesInvolvesParameter :TypeOfKernelParam ;
    :specifiesInvolvesParameterSetting :SVMKernelSetting .

:LIME
    dc:creator "Marco Tulio Ribeiro, Sameer Singh, Carlos Guestrin"@en ;
    dc:date "2016"@en ;
    dc:title "\"Why Should I Trust You?\": Explaining the Predictions of Any Classifier"@en ;
    gufo:hasReifiedQualityValue :ExplainedElementMLModel, :ExplainedElementOutput, :InputVariableWeight, :Local, :LocalFidelity, :ModelAgnostic, :Static ;
    a owl:NamedIndividual, :ExplainableAlgorithm .

:LIMEPython
    gufo:isComponentOf :ExplainWorfklow_exp2, :PythonNotebook ;
    a owl:NamedIndividual, :ExplainImplementation ;
    :executedBy :ExplainSVMLIME .

:LearningType
    a gufo:AbstractIndividualType, owl:Class, owl:NamedIndividual ;
    rdfs:label "LearningType"@en ;
    rdfs:subClassOf gufo:QualityValue .

:LimeExplanation
    gufo:wasCreatedIn :ExplainSVMLIME ;
    a owl:NamedIndividual, :ResultExplanation .

:LimeExplanation00
    gufo:isComponentOf :LimeExplanation ;
    a owl:NamedIndividual, :ExplanationComponent .

:LimeExplanation00ExplainsResultInstance00
    a owl:NamedIndividual, :ExplainsResultInstance ;
    :explainsInvolvesExplanationComponent :LimeExplanation00 ;
    :explainsInvolvesResultInstance :ResultInstance00 .

:LimeExplanation00Value
    gufo:hasQualityValue """[('intubed=1', 0.6154841019238257),
 ('icu=1', -0.23887455785695177),
 ('copd=2', -0.08853933650649158),
 ('pneumonia=1', 0.06534032643961966),
 ('patient_type=2', -0.044199746183323924),
 ('other_disease=2', 0.03710435413289758),
 ('sex=2', 0.022895460764403554),
 ('cardiovascular=2', -0.0216007102502643),
 ('hypertension=2', -0.02133577686069555),
 ('age', 0.017670861014632416),
 ('diabetes=2', 0.013580131603379215),
 ('obesity=2', -0.008897946813529133),
 ('renal_chronic=2', 0.006524385459357452),
 ('immunosuppression=2', 0.0055522636654152455),
 ('asthma=2', -0.0038508652077779717),
 ('tobacco=1', -0.003739629683093074)]"""^^xsd:string ;
    gufo:inheresIn :LimeExplanation00 ;
    a owl:NamedIndividual, :ExplanationComponentCharacteristic .

:LimeExplanation01
    gufo:isComponentOf :LimeExplanation ;
    a owl:NamedIndividual, :ExplanationComponent .

:LimeExplanation01ExplainsResultInstance01
    a owl:NamedIndividual, :ExplainsResultInstance ;
    :explainsInvolvesExplanationComponent :LimeExplanation01 ;
    :explainsInvolvesResultInstance :ResultInstance01 .

:LimeExplanation01Value
    gufo:hasQualityValue """[('intubed=97', -0.7656389673350394),
 ('icu=97', 0.23244674630754567),
 ('pneumonia=2', -0.04132288409459061),
 ('renal_chronic=2', -0.03678550151854597),
 ('patient_type=1', 0.03123426758590798),
 ('copd=2', -0.02802099547763556),
 ('other_disease=2', 0.021728249446465977),
 ('age', 0.019452275259615074),
 ('immunosuppression=2', -0.014022341322546258),
 ('hypertension=2', -0.009981418086365067),
 ('diabetes=2', 0.009679542693044097),
 ('cardiovascular=2', 0.009586878971084787),
 ('asthma=2', -0.007018022837506875),
 ('tobacco=2', 0.005437268740498237),
 ('sex=2', 0.004388335576254076),
 ('obesity=2', -0.0036122633993878363)]"""^^xsd:string ;
    gufo:inheresIn :LimeExplanation01 ;
    a owl:NamedIndividual, :ExplanationComponentCharacteristic .

:LimeExplanation02
    gufo:isComponentOf :LimeExplanation ;
    a owl:NamedIndividual, :ExplanationComponent .

:LimeExplanation02ExplainsResultInstance02
    a owl:NamedIndividual, :ExplainsResultInstance ;
    :explainsInvolvesExplanationComponent :LimeExplanation02 ;
    :explainsInvolvesResultInstance :ResultInstance02 .

:LimeExplanation02Value
    gufo:hasQualityValue """[('intubed=2', 0.7146535313854077),
 ('icu=2', -0.2363451455785819),
 ('pneumonia=1', 0.04434876291854826),
 ('patient_type=2', -0.03187719393662432),
 ('copd=2', -0.02804977874435309),
 ('immunosuppression=2', -0.022208146202334546),
 ('renal_chronic=2', -0.022061568725089225),
 ('age', 0.020898999580094297),
 ('hypertension=2', -0.018977262525854095),
 ('cardiovascular=2', 0.01665622517135697),
 ('other_disease=2', 0.015366885129255355),
 ('tobacco=2', 0.014179436848327712),
 ('asthma=2', -0.013258320905381867),
 ('diabetes=1', -0.007404500795270865),
 ('sex=1', -0.005620660391282329),
 ('obesity=2', 0.0006955766493285971)]"""^^xsd:string ;
    gufo:inheresIn :LimeExplanation02 ;
    a owl:NamedIndividual, :ExplanationComponentCharacteristic .

:LimeExplanation03
    gufo:isComponentOf :LimeExplanation ;
    a owl:NamedIndividual, :ExplanationComponent .

:LimeExplanation03ExplainsResultInstance03
    a owl:NamedIndividual, :ExplainsResultInstance ;
    :explainsInvolvesExplanationComponent :LimeExplanation03 ;
    :explainsInvolvesResultInstance :ResultInstance03 .

:LimeExplanation03Value
    gufo:hasQualityValue """[('intubed=97', -0.7657390082015048),
 ('icu=97', 0.23083196584618196),
 ('pneumonia=2', -0.04523399228398043),
 ('renal_chronic=2', -0.03566811042425281),
 ('patient_type=1', 0.03377383370054058),
 ('copd=2', -0.031095086818593427),
 ('other_disease=2', 0.022453837557559534),
 ('age', 0.02205468284021284),
 ('immunosuppression=2', -0.0142447031573384),
 ('cardiovascular=2', 0.01399767935844397),
 ('hypertension=2', -0.010628509224517354),
 ('diabetes=2', 0.010100616877406744),
 ('tobacco=2', 0.007023181169454146),
 ('sex=1', -0.0057826838110762715),
 ('asthma=2', -0.003736137355981059),
 ('obesity=2', -0.0034526460170110867)]"""^^xsd:string ;
    gufo:inheresIn :LimeExplanation03 ;
    a owl:NamedIndividual, :ExplanationComponentCharacteristic .

:LimePythonImplementsLime
    a owl:NamedIndividual, :Implements ;
    :implementsInvolvesAlgorithm :LIME ;
    :implementsInvolvesImplementation :LIMEPython .

:Local
    a owl:NamedIndividual, :ExplanationScope ;
    rdfs:comment "Indicates that the scope of the explainable method is local, that is, considers the only one instance of the dataset." .

:LocalFidelity
    a owl:NamedIndividual, :ExplanationFidelity ;
    rdfs:comment "Indicates if the explanation if locally faithfull to the underlying ML model." .

:MLAlgorithm
    a gufo:SubKind, owl:Class, owl:NamedIndividual ;
    rdfs:comment "Machine Learnin Algorithm (MLAlgorithm) is a specific type of algorithms that are used to perform machine learning, such as NN, SVM, Decision Trees, Logistic Regression"@en ;
    rdfs:label "MLAlgorithm"@en ;
    rdfs:subClassOf :Algorithm .

:MLImplementation
    a gufo:SubKind, owl:Class, owl:NamedIndividual ;
    rdfs:comment "Specific type of implementation that implements Machine Learning Algorithms."@en ;
    rdfs:label "MLImplementation"@en ;
    rdfs:subClassOf :Implementation .

:MLModel
    a gufo:Kind, owl:Class, owl:NamedIndividual ;
    rdfs:comment "Machine Learning Model (MLModel) is a generalization of a set of training data able to predict values for unseen instances. It is an output from the Train operation, which executes a ML algorithm implementation. Models have a dual nature. They can be treated as data structures and as such represented, stored and manipulated. On the other hand, they act as functions and are executed, taking as input data examples and giving as output the result of applying the function to a data example. Models can also be divided into global or local ones. A global model has global coverage of a data set, i.e., it generalizes the whole data set. A local model, such as a pattern set, is a set of local hypotheses, i.e. each applies to a limited region of the data set."@en ;
    rdfs:label "MLModel"@en ;
    rdfs:subClassOf :Output, [
        a owl:Restriction ;
        owl:onProperty [
            owl:inverseOf gufo:inheresIn
        ] ;
        owl:someValuesFrom :ModelCharacteristic
    ], [
        a owl:Restriction ;
        owl:onClass :Train ;
        owl:onProperty gufo:wasCreatedIn ;
        owl:qualifiedCardinality "1"^^xsd:nonNegativeInteger
    ] .

:MLTechnique
    a owl:Class ;
    rdfs:comment "Type of technique used by ML Algorithm."@en ;
    rdfs:label "MLTechnique"@en ;
    rdfs:subClassOf gufo:QualityValue .

:MLWorkflow
    dc:creator "Patricia"^^xsd:string ;
    gufo:participatedIn :MLWorkflow_exec ;
    a owl:NamedIndividual, :Workflow ;
    rdfs:comment "Workflow that contains the implementation steps of the ML process, executed by WFExecution."^^xsd:string .

:MLWorkflow_exec
    dc:creator "Patricia"^^xsd:string ;
    gufo:hasBeginPointInXSDDate "26-05-2021"^^xsd:date ;
    gufo:hasEndPointInXSDDate "26-05-2021"^^xsd:date ;
    gufo:isEventProperPartOf :Experiment1, :Experiment2 ;
    a owl:NamedIndividual, :WFExecution ;
    rdfs:comment "Workflow for the ML process, consisting of preprocessing data, train ML model and test the ML model."^^xsd:string .

:MachineLearningTechnique
    a gufo:AbstractIndividualType, owl:NamedIndividual .

:MeasureValue
    a gufo:SubKind, owl:Class, owl:NamedIndividual ;
    rdfs:comment "Receives the value for the measurement after the ML evaluation step is performed."@en ;
    rdfs:label "MeasureValue"@en ;
    rdfs:subClassOf :ModelEvaluationCharacteristic .

:ModelAgnostic
    a owl:NamedIndividual, :ExplainableMethodFlexibility ;
    rdfs:comment "Indicates if the explainable method is model-agnostic." .

:ModelCharacteristic
    a gufo:Kind, owl:Class, owl:NamedIndividual ;
    rdfs:comment "Characteristics of the ML model."@en ;
    rdfs:label "ModelCharacteristic"@en ;
    rdfs:subClassOf gufo:Quality, [
        a owl:Restriction ;
        owl:minQualifiedCardinality "1"^^xsd:nonNegativeInteger ;
        owl:onClass :MLModel ;
        owl:onProperty gufo:inheresIn
    ] .

:ModelEvaluation
    a gufo:Kind, owl:Class, owl:NamedIndividual ;
    rdfs:comment "ModelEvaluation is a setting of a value of the performance measure specified by the evaluation specification. It connects a evaluation measure with its value."@en ;
    rdfs:label "ModelEvaluation"@en ;
    rdfs:subClassOf :Output, [
        a owl:Restriction ;
        owl:onProperty [
            owl:inverseOf gufo:mediates
        ] ;
        owl:someValuesFrom :SpecifiesModelEvaluation
    ], [
        a owl:Restriction ;
        owl:onClass :EvaluateModel ;
        owl:onProperty gufo:wasCreatedIn ;
        owl:qualifiedCardinality "1"^^xsd:nonNegativeInteger
    ], [
        a owl:Restriction ;
        owl:onClass :Assesses ;
        owl:onProperty [
            owl:inverseOf gufo:mediates
        ] ;
        owl:qualifiedCardinality "1"^^xsd:nonNegativeInteger
    ] .

:ModelEvaluationAssessesSVMModel
    a owl:NamedIndividual, :Assesses ;
    :assessesInvolvesModel :SVMModel ;
    :assessesInvolvesModelEvaluation :SVMEvaluation .

:ModelEvaluationCharacteristic
    a gufo:Kind, owl:Class, owl:NamedIndividual ;
    rdfs:comment "Characteristics of the ML model evaluation."@en ;
    rdfs:label "ModelEvaluationCharacteristic"@en ;
    rdfs:subClassOf gufo:Quality, [
        a owl:Restriction ;
        owl:minQualifiedCardinality "1"^^xsd:nonNegativeInteger ;
        owl:onClass :SpecifiesModelEvaluation ;
        owl:onProperty gufo:inheresIn
    ] .

:ModelExplanation
    a gufo:Role, owl:Class, owl:NamedIndividual ;
    rdfs:comment "Specific type of explanation, which can focus on explaining the fitted MLModel by expressing the logic behind it."@en ;
    rdfs:label "ModelExplanation"@en ;
    rdfs:subClassOf :Explanation, [
        a owl:Restriction ;
        owl:onClass :ExplainsModel ;
        owl:onProperty [
            owl:inverseOf gufo:mediates
        ] ;
        owl:qualifiedCardinality "1"^^xsd:nonNegativeInteger
    ] .

:ModelSpecific
    a owl:NamedIndividual, :ExplainableMethodFlexibility ;
    rdfs:comment "Indicates if the explainable method is model-specific." .

:NaturalLanguage
    a owl:NamedIndividual, :ExplanationFormat ;
    rdfs:comment "Indicates that the explainable method generates explanations in the format of natural language." .

:NewValueColumnParam
    a owl:NamedIndividual, :Parameter ;
    rdfs:comment "String containing the new values for the columns to be used as parameter of a function."^^xsd:string .

:NewValueSpecifiesNewValueSetting
    a owl:NamedIndividual, :SpecifiesParameter ;
    :specifiesInvolvesParameter :NewValueColumnParam ;
    :specifiesInvolvesParameterSetting :RenameColumnNewValueSetting .

:NumberCategories
    a gufo:SubKind, owl:NamedIndividual .

:NumberFeatures
    a gufo:SubKind, owl:Class, owl:NamedIndividual ;
    rdfs:comment "Indicates the number of features that a dataset contains."@en ;
    rdfs:label "NumberFeatures"@en ;
    rdfs:subClassOf :DataCharacteristic .

:NumberInstances
    a gufo:SubKind, owl:Class, owl:NamedIndividual ;
    rdfs:comment "Indicates the number of instances that a dataset contains."@en ;
    rdfs:label "NumberInstances"@en ;
    rdfs:subClassOf :DataCharacteristic .

:NumberNulls
    a gufo:SubKind, owl:Class, owl:NamedIndividual ;
    rdfs:comment "Number of NULL values in a feature."@en ;
    rdfs:label "NumberNulls"@en ;
    rdfs:subClassOf :FeatureCharacteristic .

:Obesity_Covid-19
    gufo:hasReifiedQualityValue :Categorical ;
    gufo:isComponentOf :Covid-19 ;
    a owl:NamedIndividual, :Feature ;
    rdfs:comment "OBESITY Identifies if the patient is diagnosed with obesity."@en .

:Obesity_Covid-19Test
    gufo:hasReifiedQualityValue :Categorical ;
    gufo:isComponentOf :Covid-19TestData ;
    a owl:NamedIndividual, :Feature ;
    rdfs:comment "OBESITY Identifies if the patient is diagnosed with obesity."@en .

:Obesity_Covid-19Test_categories
    gufo:hasQualityValue "1 = Yes , 2 = No"^^xsd:string ;
    gufo:inheresIn :Obesity_Covid-19Test ;
    a owl:NamedIndividual, :Categories .

:Obesity_Covid-19Train
    gufo:hasReifiedQualityValue :Categorical ;
    gufo:isComponentOf :Covid-19TrainData ;
    a owl:NamedIndividual, :Feature ;
    rdfs:comment "OBESITY Identifies if the patient is diagnosed with obesity."@en .

:Obesity_Covid-19Train_1
    gufo:hasQualityValue 1229 ;
    gufo:inheresIn :Obesity_Covid-19Train ;
    a owl:NamedIndividual, :CategoryQuantity .

:Obesity_Covid-19Train_2
    gufo:hasQualityValue 5386 ;
    gufo:inheresIn :Obesity_Covid-19Train ;
    a owl:NamedIndividual, :CategoryQuantity .

:Obesity_Covid-19Train_categories
    gufo:hasQualityValue "1 = Yes , 2 = No"^^xsd:string ;
    gufo:inheresIn :Obesity_Covid-19Train ;
    a owl:NamedIndividual, :Categories .

:Obesity_Covid-19_1
    gufo:hasQualityValue 92272 ;
    gufo:inheresIn :Obesity_Covid-19 ;
    a owl:NamedIndividual, :CategoryQuantity .

:Obesity_Covid-19_2
    gufo:hasQualityValue 472549 ;
    gufo:inheresIn :Obesity_Covid-19 ;
    a owl:NamedIndividual, :CategoryQuantity .

:Obesity_Covid-19_Null
    gufo:hasQualityValue 1781 ;
    gufo:inheresIn :Obesity_Covid-19 ;
    a owl:NamedIndividual, :NumberNulls .

:Obesity_Covid-19_categories
    gufo:hasQualityValue "1 = Yes, 2 = No"^^xsd:string ;
    gufo:inheresIn :Obesity_Covid-19 ;
    a owl:NamedIndividual, :Categories .

:Operation
    a gufo:EventType, owl:Class, owl:NamedIndividual ;
    rdfs:comment "Operation, similarly to [DMOP] is an execution of an implementation that accomplish a specific piece of work that needs to be addressed. It is limited in time (has a start and end point), can be successful or failed."@en ;
    rdfs:label "Operation"@en ;
    rdfs:subClassOf gufo:Event, [
        a owl:Restriction ;
        owl:onProperty gufo:isEventProperPartOf ;
        owl:someValuesFrom :WFExecution
    ], [
        a owl:Restriction ;
        owl:onProperty [
            owl:inverseOf gufo:wasCreatedIn
        ] ;
        owl:someValuesFrom :Output
    ], [
        a owl:Restriction ;
        owl:minQualifiedCardinality "1"^^xsd:nonNegativeInteger ;
        owl:onClass :Implementation ;
        owl:onProperty [
            owl:inverseOf gufo:participatedIn
        ]
    ] .

:OtherDisease_Covid-19
    gufo:hasReifiedQualityValue :Categorical ;
    gufo:isComponentOf :Covid-19 ;
    a owl:NamedIndividual, :Feature ;
    rdfs:comment "Identifies if the patient has a diagnosis of other diseases."@en .

:OtherDisease_Covid-19Test
    gufo:hasReifiedQualityValue :Categorical ;
    gufo:isComponentOf :Covid-19TestData ;
    a owl:NamedIndividual, :Feature ;
    rdfs:comment "Identifies if the patient has a diagnosis of other diseases."@en .

:OtherDisease_Covid-19Test_categories
    gufo:hasQualityValue "1 = Yes , 2 = No"^^xsd:string ;
    gufo:inheresIn :OtherDisease_Covid-19Test ;
    a owl:NamedIndividual, :Categories .

:OtherDisease_Covid-19Train
    gufo:hasReifiedQualityValue :Categorical ;
    gufo:isComponentOf :Covid-19TrainData ;
    a owl:NamedIndividual, :Feature ;
    rdfs:comment "Identifies if the patient has a diagnosis of other diseases."@en .

:OtherDisease_Covid-19Train_1
    gufo:hasQualityValue 185 ;
    gufo:inheresIn :OtherDisease_Covid-19Train ;
    a owl:NamedIndividual, :CategoryQuantity .

:OtherDisease_Covid-19Train_2
    gufo:hasQualityValue 6422 ;
    gufo:inheresIn :OtherDisease_Covid-19Train ;
    a owl:NamedIndividual, :CategoryQuantity .

:OtherDisease_Covid-19Train_Null
    gufo:hasQualityValue 8 ;
    gufo:inheresIn :OtherDisease_Covid-19Train ;
    a owl:NamedIndividual, :NumberNulls .

:OtherDisease_Covid-19Train_categories
    gufo:hasQualityValue "1 = Yes , 2 = No"^^xsd:string ;
    gufo:inheresIn :OtherDisease_Covid-19Train ;
    a owl:NamedIndividual, :Categories .

:OtherDisease_Covid-19_1
    gufo:hasQualityValue 17084 ;
    gufo:inheresIn :OtherDisease_Covid-19 ;
    a owl:NamedIndividual, :CategoryQuantity .

:OtherDisease_Covid-19_2
    gufo:hasQualityValue 546920 ;
    gufo:inheresIn :OtherDisease_Covid-19 ;
    a owl:NamedIndividual, :CategoryQuantity .

:OtherDisease_Covid-19_Null
    gufo:hasQualityValue 2598 ;
    gufo:inheresIn :OtherDisease_Covid-19 ;
    a owl:NamedIndividual, :NumberNulls .

:OtherDisease_Covid-19_categories
    gufo:hasQualityValue "1 = Yes, 2 = No"^^xsd:string ;
    gufo:inheresIn :OtherDisease_Covid-19 ;
    a owl:NamedIndividual, :Categories .

:Output
    a gufo:Category, owl:Class, owl:NamedIndividual ;
    rdfs:comment "Artifact created in the Operation, which is the event that brought the output into existence. It can be a preprocessed dataset, a machine learning model, an evaluation."@en ;
    rdfs:label "Output"@en ;
    rdfs:subClassOf gufo:FunctionalComplex, [
        a owl:Restriction ;
        owl:onClass :Operation ;
        owl:onProperty gufo:wasCreatedIn ;
        owl:qualifiedCardinality "1"^^xsd:nonNegativeInteger
    ] .

:Parameter
    a gufo:Kind, owl:Class, owl:NamedIndividual ;
    rdfs:comment "Prior parameter of an implementation, i.e., a parameter which is set before its execution. For example, a Hyperparameter when training a ML model."@en ;
    rdfs:label "Parameter"@en ;
    rdfs:subClassOf gufo:FunctionalComplex, [
        a owl:Restriction ;
        owl:onProperty [
            owl:inverseOf gufo:mediates
        ] ;
        owl:someValuesFrom :HasParameter
    ], [
        a owl:Restriction ;
        owl:onClass :SpecifiesParameter ;
        owl:onProperty [
            owl:inverseOf gufo:mediates
        ] ;
        owl:qualifiedCardinality "1"^^xsd:nonNegativeInteger
    ] .

:ParameterSetting
    a gufo:Kind, owl:Class, owl:NamedIndividual ;
    rdfs:comment "ParameterSetting is an entity which connects a parameter and its value that is being set before an implementation execution."@en ;
    rdfs:label "ParameterSetting"@en ;
    rdfs:subClassOf gufo:FunctionalComplex, [
        a owl:Restriction ;
        owl:onClass :ParameterSettingCharacteristic ;
        owl:onProperty [
            owl:inverseOf gufo:inheresIn
        ] ;
        owl:qualifiedCardinality "1"^^xsd:nonNegativeInteger
    ], [
        a owl:Restriction ;
        owl:onClass :SpecifiesParameter ;
        owl:onProperty [
            owl:inverseOf gufo:mediates
        ] ;
        owl:qualifiedCardinality "1"^^xsd:nonNegativeInteger
    ], [
        a owl:Restriction ;
        owl:onClass :Operation ;
        owl:onProperty gufo:participatedIn ;
        owl:qualifiedCardinality "1"^^xsd:nonNegativeInteger
    ] .

:ParameterSettingCharacteristic
    a gufo:Kind, owl:Class, owl:NamedIndividual ;
    rdfs:comment "Characteristics of the parameter setting."@en ;
    rdfs:label "ParameterSettingCharacteristic"@en ;
    rdfs:subClassOf gufo:Quality, [
        a owl:Restriction ;
        owl:minQualifiedCardinality "1"^^xsd:nonNegativeInteger ;
        owl:onClass :ParameterSetting ;
        owl:onProperty gufo:inheresIn
    ] .

:ParameterSettingValue
    a gufo:SubKind, owl:Class, owl:NamedIndividual ;
    rdfs:comment "Receives the value of the parameter set before the execution of the implementation takes place."@en ;
    rdfs:label "ParameterSettingValue"@en ;
    rdfs:subClassOf :ParameterSettingCharacteristic .

:PatientType_Covid-19
    gufo:hasReifiedQualityValue :Categorical ;
    gufo:isComponentOf :Covid-19 ;
    a owl:NamedIndividual, :Feature ;
    rdfs:comment "PATIENT_TYPE Identifies the type of care received by the patient in the unit. It is called an outpatient if you returned home or it is called an inpatient if you were admitted to hospital."@en .

:PatientType_Covid-19Test
    gufo:hasReifiedQualityValue :Categorical ;
    gufo:isComponentOf :Covid-19TestData ;
    a owl:NamedIndividual, :Feature ;
    rdfs:comment "Identifies if the patient returned home or were admitted to hospital."@en .

:PatientType_Covid-19Test_categories
    gufo:hasQualityValue "1 = Ambulatory , 2 = Hospitalized"^^xsd:string ;
    gufo:inheresIn :PatientType_Covid-19Test ;
    a owl:NamedIndividual, :Categories .

:PatientType_Covid-19Train
    gufo:hasReifiedQualityValue :Categorical ;
    gufo:isComponentOf :Covid-19TrainData ;
    a owl:NamedIndividual, :Feature ;
    rdfs:comment "Identifies it the patient returned home or were admitted to hospital."@en .

:PatientType_Covid-19Train_categories
    gufo:hasQualityValue "1 = Ambulatory , 2 = Hospitalized"^^xsd:string ;
    gufo:inheresIn :PatientType_Covid-19Train ;
    a owl:NamedIndividual, :Categories .

:PatientType_Covid-19_1
    gufo:hasQualityValue 444689 ;
    gufo:inheresIn :PatientType_Covid-19 ;
    a owl:NamedIndividual, :CategoryQuantity .

:PatientType_Covid-19_2
    gufo:hasQualityValue 121913 ;
    gufo:inheresIn :PatientType_Covid-19 ;
    a owl:NamedIndividual, :CategoryQuantity .

:PatientType_Covid-19_categories
    gufo:hasQualityValue "1=Ambulatory, 2=Hospitalized"^^xsd:string ;
    gufo:inheresIn :PatientType_Covid-19 ;
    a owl:NamedIndividual, :Categories .

:Pneumona_Covid-19_2
    gufo:hasQualityValue 478416 ;
    gufo:inheresIn :Pneumonia_Covid-19 ;
    a owl:NamedIndividual, :CategoryQuantity .

:Pneumonia_Covid-19
    gufo:hasReifiedQualityValue :Categorical ;
    gufo:isComponentOf :Covid-19 ;
    a owl:NamedIndividual, :Feature ;
    rdfs:comment "PNEUMONIA Identifies if the patient was diagnosed with pneumonia."@en .

:Pneumonia_Covid-19Test
    gufo:hasReifiedQualityValue :Categorical ;
    gufo:isComponentOf :Covid-19TestData ;
    a owl:NamedIndividual, :Feature ;
    rdfs:comment "PNEUMONIA Identifies if the patient was diagnosed with pneumonia."@en .

:Pneumonia_Covid-19Test_categories
    gufo:hasQualityValue "1 = Yes , 2 = No"^^xsd:string ;
    gufo:inheresIn :Pneumonia_Covid-19Test ;
    a owl:NamedIndividual, :Categories .

:Pneumonia_Covid-19Train
    gufo:hasReifiedQualityValue :Categorical ;
    gufo:isComponentOf :Covid-19TrainData ;
    a owl:NamedIndividual, :Feature ;
    rdfs:comment "PNEUMONIA Identifies if the patient was diagnosed with pneumonia."@en .

:Pneumonia_Covid-19Train_1
    gufo:hasQualityValue 1394 ;
    gufo:inheresIn :Pneumonia_Covid-19Train ;
    a owl:NamedIndividual, :CategoryQuantity .

:Pneumonia_Covid-19Train_2
    gufo:hasQualityValue 5221 ;
    gufo:inheresIn :Pneumonia_Covid-19Train ;
    a owl:NamedIndividual, :CategoryQuantity .

:Pneumonia_Covid-19Train_categories
    gufo:hasQualityValue "1 = Yes , 2 = No"^^xsd:string ;
    gufo:inheresIn :Pneumonia_Covid-19Train ;
    a owl:NamedIndividual, :Categories .

:Pneumonia_Covid-19_1
    gufo:hasQualityValue 88175 ;
    gufo:inheresIn :Pneumonia_Covid-19 ;
    a owl:NamedIndividual, :CategoryQuantity .

:Pneumonia_Covid-19_Null
    gufo:hasQualityValue 11 ;
    gufo:inheresIn :Pneumonia_Covid-19 ;
    a owl:NamedIndividual, :NumberNulls .

:Pneumonia_Covid-19_categories
    gufo:hasQualityValue "1 = Yes, 2 = No"^^xsd:string ;
    gufo:inheresIn :Pneumonia_Covid-19 ;
    a owl:NamedIndividual, :Categories .

:Predict
    a owl:Class ;
    rdfs:comment "Specific type of operation that executes the PredictImplementation, generating results from the test data."@en ;
    rdfs:label "Predict"@en ;
    rdfs:subClassOf :Operation, [
        a owl:Restriction ;
        owl:onProperty [
            owl:inverseOf gufo:participatedIn
        ] ;
        owl:someValuesFrom :TestData
    ], [
        a owl:Restriction ;
        owl:minQualifiedCardinality "1"^^xsd:nonNegativeInteger ;
        owl:onClass :PredictImplementation ;
        owl:onProperty [
            owl:inverseOf gufo:participatedIn
        ]
    ], [
        a owl:Restriction ;
        owl:onClass :Train ;
        owl:onProperty gufo:historicallyDependsOn ;
        owl:qualifiedCardinality "1"^^xsd:nonNegativeInteger
    ], [
        a owl:Restriction ;
        owl:onClass :Result ;
        owl:onProperty [
            owl:inverseOf gufo:wasCreatedIn
        ] ;
        owl:qualifiedCardinality "1"^^xsd:nonNegativeInteger
    ] .

:PredictImplementation
    a gufo:SubKind, owl:Class, owl:NamedIndividual ;
    rdfs:comment "Specific type of implementation that implements the code to generate predictions/results by calling the function of the fitted MLModel."@en ;
    rdfs:label "PredictImplementation"@en ;
    rdfs:subClassOf :Implementation, [
        a owl:Restriction ;
        owl:onClass :Calls ;
        owl:onProperty [
            owl:inverseOf gufo:mediates
        ] ;
        owl:qualifiedCardinality "1"^^xsd:nonNegativeInteger
    ] .

:PredictImplementationCallsSVMModel
    a owl:NamedIndividual, :Calls ;
    :callsInvolvesMLModel :SVMModel ;
    :callsInvolvesPredictImplementation :PredictSVMPython .

:PredictSVMPython
    dc:creator "Scikit-learn: Machine Learning in Python, Pedregosa et al., JMLR 12, pp. 2825-2830, 2011."^^xsd:string ;
    gufo:isComponentOf :ExplainWorkflow_exp1, :MLWorkflow, :PythonNotebook ;
    a owl:NamedIndividual, :PredictImplementation ;
    rdfs:comment "Implementation of the predict function  in Python to predict the results of a dataset using the fitted ML model."^^xsd:string ;
    :executedBy :PredictTest, :PredictTrain_exp1 .

:PredictSVMPythonFromLibrary
    dc:creator "Scikit-learn: Machine Learning in Python, Pedregosa et al., JMLR 12, pp. 2825-2830, 2011."^^xsd:string ;
    gufo:hasQualityValue "scikit-learn"^^xsd:string ;
    gufo:inheresIn :PredictSVMPython ;
    a owl:NamedIndividual, :ImplementationLibrary .

:PredictTest
    dc:creator "Patricia"^^xsd:string ;
    gufo:historicallyDependsOn :TrainSVM ;
    gufo:isEventProperPartOf :MLWorkflow_exec ;
    a owl:NamedIndividual, :Predict ;
    rdfs:comment "Generate predicitions (classifications) using the test dataset in the ML workflow to test the ML Model."^^xsd:string .

:PredictTrain_exp1
    dc:creator "Patricia"^^xsd:string ;
    gufo:historicallyDependsOn :TrainSVM ;
    gufo:isEventProperPartOf :ExplainWorkflow_exec_exp1 ;
    a owl:NamedIndividual, :Predict ;
    rdfs:comment "Generate predicitions (classifications) using the train dataset in the Explanation workflow to generate explanations."^^xsd:string .

:Pregnacy_Covid-19_Null
    gufo:hasQualityValue 1587 ;
    gufo:inheresIn :Pregnant_Covid-19 ;
    a owl:NamedIndividual, :NumberNulls .

:Pregnancy_Covid-19_1
    gufo:hasQualityValue 4063 ;
    gufo:inheresIn :Pregnant_Covid-19 ;
    a owl:NamedIndividual, :CategoryQuantity .

:Pregnancy_Covid-19_2
    gufo:hasQualityValue 273840 ;
    gufo:inheresIn :Pregnant_Covid-19 ;
    a owl:NamedIndividual, :CategoryQuantity .

:Pregnancy_Covid-19_97
    gufo:hasQualityValue 287112 ;
    gufo:inheresIn :Pregnant_Covid-19 ;
    a owl:NamedIndividual, :CategoryQuantity .

:Pregnant_Covid-19
    gufo:hasReifiedQualityValue :Categorical ;
    gufo:isComponentOf :Covid-19 ;
    a owl:NamedIndividual, :Feature ;
    rdfs:comment "Identifies if the patient is pregnant."@en .

:Pregnant_Covid-19_categories
    gufo:hasQualityValue "1 = Yes, 2 = No, 97 = Not applicable"^^xsd:string ;
    gufo:inheresIn :Pregnant_Covid-19 ;
    a owl:NamedIndividual, :Categories .

:Preprocess
    a gufo:EventType, owl:Class, owl:NamedIndividual ;
    rdfs:comment "Specific type of operation that focus on preprocessing the input data to make it more adequate to train and test the ML model."@en ;
    rdfs:label "Preprocess"@en ;
    rdfs:subClassOf :Operation, [
        a owl:Restriction ;
        owl:onProperty [
            owl:inverseOf gufo:participatedIn
        ] ;
        owl:someValuesFrom :InputData
    ], [
        a owl:Restriction ;
        owl:onProperty [
            owl:inverseOf gufo:wasCreatedIn
        ] ;
        owl:someValuesFrom :PreprocessedData
    ], [
        a owl:Restriction ;
        owl:minQualifiedCardinality "1"^^xsd:nonNegativeInteger ;
        owl:onClass :PreprocessImplementation ;
        owl:onProperty [
            owl:inverseOf gufo:participatedIn
        ]
    ] .

:PreprocessCovid
    dc:creator "Patricia"^^xsd:string ;
    gufo:isEventProperPartOf :MLWorkflow_exec ;
    a owl:NamedIndividual, :Preprocess ;
    rdfs:comment "Preprocess Covid-19 dataset"^^xsd:string .

:PreprocessImplementation
    a gufo:SubKind, owl:Class, owl:NamedIndividual ;
    rdfs:comment "Specific type of implementation that implements preprocessing algorithms."@en ;
    rdfs:label "PreprocessImplementation"@en ;
    rdfs:subClassOf :Implementation .

:PreprocessedData
    a gufo:Phase, owl:Class, owl:NamedIndividual ;
    rdfs:comment "Type of output that is generated by the preprocessing operation. It represents the phase of the data after the preprocessing step."@en ;
    rdfs:label "PreprocessedData"@en ;
    rdfs:subClassOf :Data, :Output, [
        a owl:Restriction ;
        owl:onClass :Preprocess ;
        owl:onProperty gufo:wasCreatedIn ;
        owl:qualifiedCardinality "1"^^xsd:nonNegativeInteger
    ] .

:PreprocessingAlgorithm
    a gufo:SubKind, owl:Class, owl:NamedIndividual ;
    rdfs:comment "Specific type of algorithm that focus on preprocessing the input data making it more adequate to train and test the ML model."@en ;
    rdfs:label "PreprocessingAlgorithm"@en ;
    rdfs:subClassOf :Algorithm .

:PreprocessingTechnique
    a gufo:AbstractIndividualType, owl:Class, owl:NamedIndividual ;
    rdfs:label "PreprocessingTechnique"@en ;
    rdfs:subClassOf gufo:QualityValue .

:PythonNotebook
    a owl:NamedIndividual, :Software ;
    rdfs:comment """Software used to implement the Case study.
Jupyter Notebook 6.0.3
Python 3"""^^xsd:string .

:RIPPER
    dc:creator "William W. Cohen, Yoram Singer"^^xsd:string ;
    dc:date "1995"^^xsd:date ;
    dc:title "A Simple, Fast, and Effective Rule Learner"^^xsd:string ;
    gufo:hasReifiedQualityValue :ExplainedElementMLModel, :Global, :ModelAgnostic, :Rules, :Static, :Unfaithful ;
    a owl:NamedIndividual, :ExplainableAlgorithm .

:RIPPERExplainsSVMModel
    a owl:NamedIndividual, :ExplainsModel ;
    :explainsModelInvolvesModel :SVMModel ;
    :explainsModelInvolvesModelExplanation :RipperExplanation .

:Regression
    a owl:NamedIndividual, :MLTechnique ;
    rdfs:comment "Indicates that the ML algorithm performs regression." .

:RemoveColumnPythonFromLibrary
    dc:creator """pandas: powerful Python data analysistoolkit
Wes McKinney and the Pandas Development Team"""^^xsd:string ;
    gufo:hasQualityValue "pandas"^^xsd:string ;
    gufo:inheresIn :RemoveColumnsPython ;
    a owl:NamedIndividual, :ImplementationLibrary ;
    owl:versionInfo "Release 1.2.4"^^xsd:string .

:RemoveColumnPythonHasParameterColumn
    a owl:NamedIndividual, :HasParameter ;
    :hasParameterInvolvesImplementation :RemoveColumnsPython ;
    :hasParameterInvolvesParameter :DropColumnsParam .

:RemoveColumnSetting
    gufo:participatedIn :PreprocessCovid ;
    a owl:NamedIndividual, :ParameterSetting ;
    rdfs:comment "Indicates the columns to be removed of the dataset."^^xsd:string .

:RemoveColumnValue
    gufo:hasQualityValue "['id', 'covid_res','entry_date','date_symptoms','date_died', 'contact_other_covid', 'pregnancy']"^^xsd:string ;
    gufo:inheresIn :RemoveColumnSetting ;
    a owl:NamedIndividual, :ParameterSettingValue .

:RemoveColumnsPython
    dc:creator """pandas: powerful Python data analysis toolkit
Wes McKinney and the Pandas Development Team"""^^xsd:string ;
    gufo:isComponentOf :MLWorkflow, :PythonNotebook ;
    a owl:NamedIndividual, :PreprocessImplementation ;
    rdfs:comment "Implementation of drop function to remove columns of the dataframe in Python."^^xsd:string ;
    owl:versionInfo "Release 1.2.4"^^xsd:string ;
    :executedBy :PreprocessCovid .

:RemoveColumnsPythonImplementsDropColumn
    a owl:NamedIndividual, :Implements ;
    :implementsInvolvesAlgorithm :DropColumn ;
    :implementsInvolvesImplementation :RemoveColumnsPython .

:RemoveColumnsSpecifiesRemoveColumnSetting
    a owl:NamedIndividual, :SpecifiesParameter ;
    :specifiesInvolvesParameter :DropColumnsParam ;
    :specifiesInvolvesParameterSetting :RemoveColumnSetting .

:RenalChronic_Covid-19
    gufo:hasReifiedQualityValue :Categorical ;
    gufo:isComponentOf :Covid-19 ;
    a owl:NamedIndividual, :Feature ;
    rdfs:comment "Identifies if the patient has a diagnosis of chronic kidney failure."@en .

:RenalChronic_Covid-19Test
    gufo:hasReifiedQualityValue :Categorical ;
    gufo:isComponentOf :Covid-19TestData ;
    a owl:NamedIndividual, :Feature ;
    rdfs:comment "Identifies if the patient has a diagnosis of chronic kidney failure."@en .

:RenalChronic_Covid-19Test_categories
    gufo:hasQualityValue "1 = Yes , 2 = No"^^xsd:string ;
    gufo:inheresIn :RenalChronic_Covid-19Test ;
    a owl:NamedIndividual, :Categories .

:RenalChronic_Covid-19Train
    gufo:hasReifiedQualityValue :Categorical ;
    gufo:isComponentOf :Covid-19TrainData ;
    a owl:NamedIndividual, :Feature ;
    rdfs:comment "Identifies if the patient has a diagnosis of chronic kidney failure."@en .

:RenalChronic_Covid-19Train_1
    gufo:hasQualityValue 130 ;
    gufo:inheresIn :RenalChronic_Covid-19Train ;
    a owl:NamedIndividual, :CategoryQuantity .

:RenalChronic_Covid-19Train_2
    gufo:hasQualityValue 6485 ;
    gufo:inheresIn :RenalChronic_Covid-19Train ;
    a owl:NamedIndividual, :CategoryQuantity .

:RenalChronic_Covid-19Train_categories
    gufo:hasQualityValue "1 = Yes , 2 = No"^^xsd:string ;
    gufo:inheresIn :RenalChronic_Covid-19Train ;
    a owl:NamedIndividual, :Categories .

:RenalChronic_Covid-19_1
    gufo:hasQualityValue 11250 ;
    gufo:inheresIn :RenalChronic_Covid-19 ;
    a owl:NamedIndividual, :CategoryQuantity .

:RenalChronic_Covid-19_2
    gufo:hasQualityValue 553560 ;
    gufo:inheresIn :RenalChronic_Covid-19 ;
    a owl:NamedIndividual, :CategoryQuantity .

:RenalChronic_Covid-19_Null
    gufo:hasQualityValue 1792 ;
    gufo:inheresIn :RenalChronic_Covid-19 ;
    a owl:NamedIndividual, :NumberNulls .

:RenalChronic_Covid-19_categories
    gufo:hasQualityValue "1 = Yes, 2 = No"^^xsd:string ;
    gufo:inheresIn :RenalChronic_Covid-19 ;
    a owl:NamedIndividual, :Categories .

:RenameColumn
    gufo:hasReifiedQualityValue :TransformData ;
    a owl:NamedIndividual, :PreprocessingAlgorithm ;
    rdfs:comment "Rename columns from the dataframe."@en .

:RenameColumnNewValueSetting
    gufo:participatedIn :PreprocessCovid ;
    a owl:NamedIndividual, :ParameterSetting ;
    rdfs:comment "Indicates the columns to be renamed of the dataset."^^xsd:string .

:RenameColumnParam
    a owl:NamedIndividual, :Parameter ;
    rdfs:comment "Columns of the dataset to be removed."@en .

:RenameColumnPython
    dc:creator """pandas: powerful Python data analysis toolkit
Wes McKinney and the Pandas Development Team"""^^xsd:string ;
    gufo:isComponentOf :MLWorkflow, :PythonNotebook ;
    a owl:NamedIndividual, :PreprocessImplementation ;
    rdfs:comment "Implementation of rename function to rename columns of the dataframe in Python."^^xsd:string ;
    owl:versionInfo "Release 1.2.4"^^xsd:string ;
    :executedBy :PreprocessCovid .

:RenameColumnPythonFromLibrary
    dc:creator """pandas: powerful Python data analysistoolkit
Wes McKinney and the Pandas Development Team"""^^xsd:string ;
    gufo:hasQualityValue "pandas"^^xsd:string ;
    gufo:inheresIn :RenameColumnPython ;
    a owl:NamedIndividual, :ImplementationLibrary ;
    owl:versionInfo "Release 1.2.4"^^xsd:string .

:RenameColumnPythonHasParameterColumn
    a owl:NamedIndividual, :HasParameter ;
    :hasParameterInvolvesImplementation :RenameColumnPython ;
    :hasParameterInvolvesParameter :RenameColumnParam .

:RenameColumnPythonHasParameterNewColumn
    a owl:NamedIndividual, :HasParameter ;
    :hasParameterInvolvesImplementation :RenameColumnPython ;
    :hasParameterInvolvesParameter :NewValueColumnParam .

:RenameColumnSetting
    gufo:participatedIn :PreprocessCovid ;
    a owl:NamedIndividual, :ParameterSetting ;
    rdfs:comment "Indicates the new names for the columns to be renamed of the dataset."^^xsd:string .

:RenameColumnValue
    gufo:hasQualityValue "[inmsupr,patient_type]"^^xsd:string ;
    gufo:inheresIn :RenameColumnSetting ;
    a owl:NamedIndividual, :ParameterSettingValue .

:RenameColumnsPythonImplementsRenameColumn
    a owl:NamedIndividual, :Implements ;
    :implementsInvolvesAlgorithm :RenameColumn ;
    :implementsInvolvesImplementation :RenameColumnPython .

:RenameNewColumnValue
    gufo:hasQualityValue "[immunosuppression,hospitalized]"^^xsd:string ;
    gufo:inheresIn :RenameColumnNewValueSetting ;
    a owl:NamedIndividual, :ParameterSettingValue .

:Result
    a gufo:Kind, owl:Class, owl:NamedIndividual ;
    rdfs:comment "Type of output that is generated by the test(predict) operation. It has the results or predictions generated using the fitted MLModel on the test data."@en ;
    rdfs:label "Result"@en ;
    rdfs:subClassOf :Output, [
        a owl:Restriction ;
        owl:onClass :Predict ;
        owl:onProperty gufo:wasCreatedIn ;
        owl:qualifiedCardinality "1"^^xsd:nonNegativeInteger
    ] .

:ResultExplanation
    a gufo:Role, owl:Class, owl:NamedIndividual ;
    rdfs:comment "Specific type of explanation, which focus on explaining the result or predicitons obtained by applying the MLModel function on the test data."@en ;
    rdfs:label "ResultExplanation"@en ;
    rdfs:subClassOf :Explanation .

:ResultInstance
    a gufo:Kind, owl:Class, owl:NamedIndividual ;
    rdfs:comment "Instance that represents one result or prediction from the total results."@en ;
    rdfs:label "ResultInstance"@en ;
    rdfs:subClassOf gufo:FunctionalComplex, [
        a owl:Restriction ;
        owl:onProperty gufo:isComponentOf ;
        owl:someValuesFrom :Result
    ] .

:ResultInstance00
    gufo:isComponentOf :TestPrediction ;
    a owl:NamedIndividual, :ResultInstance ;
    rdfs:comment "Result/prediction generated using the fitted SVM model for one instance of the test dataset."^^xsd:string .

:ResultInstance01
    gufo:isComponentOf :TestPrediction ;
    a owl:NamedIndividual, :ResultInstance ;
    rdfs:comment "Result/prediction generated using the fitted SVM model for one instance of the test dataset."^^xsd:string .

:ResultInstance02
    gufo:isComponentOf :TestPrediction ;
    a owl:NamedIndividual, :ResultInstance ;
    rdfs:comment "Result/prediction generated using the fitted SVM model for one instance of the test dataset."^^xsd:string .

:ResultInstance03
    gufo:isComponentOf :TestPrediction ;
    a owl:NamedIndividual, :ResultInstance .

:ResultInstance15
    gufo:isComponentOf :TestPrediction ;
    a owl:NamedIndividual, :ResultInstance ;
    rdfs:comment "Result/prediction generated using the fitted SVM model for one instance of the test dataset."^^xsd:string .

:ResultInstance28
    gufo:isComponentOf :TestPrediction ;
    a owl:NamedIndividual, :ResultInstance ;
    rdfs:comment "Result/prediction generated using the fitted SVM model for one instance of the test dataset."^^xsd:string .

:ResultInstance46
    gufo:isComponentOf :TestPrediction ;
    a owl:NamedIndividual, :ResultInstance ;
    rdfs:comment "Result/prediction generated using the fitted SVM model for one instance of the test dataset."^^xsd:string .

:RipperEvaluation
    gufo:wasCreatedIn :EvaluateRIPPER ;
    a owl:NamedIndividual, :ExplanationEvaluation ;
    rdfs:comment "Evaluation of the explanations generated by Ripper."^^xsd:string .

:RipperExplanation
    gufo:participatedIn :EvaluateRIPPER ;
    gufo:wasCreatedIn :ExplainSVMRIPPER ;
    a owl:NamedIndividual, :ModelExplanation ;
    rdfs:comment "Rule set generated by RIPPER aims to explains the logic behind the ML model, instead of explaining a single result."^^xsd:string .

:RipperPython
    dc:creator "Ilan Moscovitz"^^xsd:string ;
    gufo:isComponentOf :ExplainWorkflow_exp1, :PythonNotebook ;
    a owl:NamedIndividual, :ExplainImplementation ;
    rdfs:comment "Implementation of the RIPPER rule extractor method in wittgenstein library in Python."^^xsd:string ;
    :executedBy :ExplainSVMRIPPER .

:RipperPythonFromLibrary
    dc:creator "Ilan Moscovitz"^^xsd:string ;
    gufo:hasQualityValue "Wittgenstein"^^xsd:string ;
    gufo:inheresIn :RipperPython ;
    a owl:NamedIndividual, :ImplementationLibrary ;
    rdfs:comment "https://github.com/imoscovitz/wittgenstein"^^xsd:string .

:RipperPythonImplementsRipper
    a owl:NamedIndividual, :Implements ;
    :implementsInvolvesAlgorithm :RIPPER ;
    :implementsInvolvesImplementation :RipperPython .

:RipperRule01
    gufo:isComponentOf :RipperExplanation ;
    a owl:NamedIndividual, :ExplanationComponent .

:RipperRule01Value
    gufo:hasQualityValue "[age=66-99 ^ pneumonia=1 ^ hypertension=1 ^ hospitalized=2 ^ sex=2]"^^xsd:string ;
    gufo:inheresIn :RipperRule01 ;
    a owl:NamedIndividual, :ExplanationComponentCharacteristic .

:RipperRule02
    gufo:isComponentOf :RipperExplanation ;
    a owl:NamedIndividual, :ExplanationComponent .

:RipperRule02Value
    gufo:hasQualityValue "[pneumonia=1 ^ age=66-99 ^ icu=2 ^ intubed=1]"^^xsd:string ;
    gufo:inheresIn :RipperRule02 ;
    a owl:NamedIndividual, :ExplanationComponentCharacteristic .

:RipperRule03
    gufo:isComponentOf :RipperExplanation ;
    a owl:NamedIndividual, :ExplanationComponent .

:RipperRule03Value
    gufo:hasQualityValue "[pneumonia=1 ^ age=66-99 ^ icu=2 ^ hypertension=1 ^ asthma=2 ^ copd=1]"^^xsd:string ;
    gufo:inheresIn :RipperRule03 ;
    a owl:NamedIndividual, :ExplanationComponentCharacteristic .

:RipperRule04
    gufo:isComponentOf :RipperExplanation ;
    a owl:NamedIndividual, :ExplanationComponent .

:RipperRule04Value
    gufo:hasQualityValue "[pneumonia=1 ^ age=66-99 ^ icu=2 ^ hypertension=1]"^^xsd:string ;
    gufo:inheresIn :RipperRule04 ;
    a owl:NamedIndividual, :ExplanationComponentCharacteristic .

:RipperRule05
    gufo:isComponentOf :RipperExplanation ;
    a owl:NamedIndividual, :ExplanationComponent .

:RipperRule05Value
    gufo:hasQualityValue "[pneumonia=1 ^ intubed=1 ^ icu=2]"^^xsd:string ;
    gufo:inheresIn :RipperRule05 ;
    a owl:NamedIndividual, :ExplanationComponentCharacteristic .

:RipperRule06
    gufo:isComponentOf :RipperExplanation ;
    a owl:NamedIndividual, :ExplanationComponent .

:RipperRule06Value
    gufo:hasQualityValue "[pneumonia=1 ^ age=66-99 ^ icu=2 ^ sex=2]"^^xsd:string ;
    gufo:inheresIn :RipperRule06 ;
    a owl:NamedIndividual, :ExplanationComponentCharacteristic .

:RipperRule07
    gufo:isComponentOf :RipperExplanation ;
    a owl:NamedIndividual, :ExplanationComponent .

:RipperRule07Value
    gufo:hasQualityValue "[renal_chronic=1 ^ pneumonia=1 ^ hospitalized=2 ^ sex=2]"^^xsd:string ;
    gufo:inheresIn :RipperRule07 ;
    a owl:NamedIndividual, :ExplanationComponentCharacteristic .

:RipperRule08
    gufo:isComponentOf :RipperExplanation ;
    a owl:NamedIndividual, :ExplanationComponent .

:RipperRule08Value
    gufo:hasQualityValue "[pneumonia=1 ^ age=66-99 ^ intubed=1]"^^xsd:string ;
    gufo:inheresIn :RipperRule08 ;
    a owl:NamedIndividual, :ExplanationComponentCharacteristic .

:RipperRule09
    gufo:isComponentOf :RipperExplanation ;
    a owl:NamedIndividual, :ExplanationComponent .

:RipperRule09Value
    gufo:hasQualityValue ""^^xsd:string ;
    gufo:inheresIn :RipperRule09 ;
    a owl:NamedIndividual, :ExplanationComponentCharacteristic .

:RipperRule10
    gufo:isComponentOf :RipperExplanation ;
    a owl:NamedIndividual, :ExplanationComponent .

:RipperRule10Value
    gufo:hasQualityValue "[pneumonia=1 ^ age=66-99 ^ renal_chronic=1]"^^xsd:string ;
    gufo:inheresIn :RipperRule10 ;
    a owl:NamedIndividual, :ExplanationComponentCharacteristic .

:RipperRule11
    gufo:isComponentOf :RipperExplanation ;
    a owl:NamedIndividual, :ExplanationComponent .

:RipperRule11Value
    gufo:hasQualityValue "[hospitalized=2 ^ renal_chronic=1 ^ other_disease=1]"^^xsd:string ;
    gufo:inheresIn :RipperRule11 ;
    a owl:NamedIndividual, :ExplanationComponentCharacteristic .

:RipperRule12
    gufo:isComponentOf :RipperExplanation ;
    a owl:NamedIndividual, :ExplanationComponent .

:RipperRule12Value
    gufo:hasQualityValue "[pneumonia=1 ^ renal_chronic=1 ^ age=51-57]"^^xsd:string ;
    gufo:inheresIn :RipperRule12 ;
    a owl:NamedIndividual, :ExplanationComponentCharacteristic .

:RipperRule13
    gufo:isComponentOf :RipperExplanation ;
    a owl:NamedIndividual, :ExplanationComponent .

:RipperRule13Value
    gufo:hasQualityValue "[icu=2 ^ age=66-99 ^ renal_chronic=1]"^^xsd:string ;
    gufo:inheresIn :RipperRule13 ;
    a owl:NamedIndividual, :ExplanationComponentCharacteristic .

:RipperRule14
    gufo:isComponentOf :RipperExplanation ;
    a owl:NamedIndividual, :ExplanationComponent .

:RipperRule14Value
    gufo:hasQualityValue "[pneumonia=1 ^ hypertension=1 ^ age=57-66 ^ sex=2 ^ intubed=1]"^^xsd:string ;
    gufo:inheresIn :RipperRule14 ;
    a owl:NamedIndividual, :ExplanationComponentCharacteristic .

:RipperRule15
    gufo:isComponentOf :RipperExplanation ;
    a owl:NamedIndividual, :ExplanationComponent .

:RipperRule15Value
    gufo:hasQualityValue "[age=57-66 ^ hypertension=1 ^ pneumonia=1 ^ diabetes=2 ^ sex=2 ^ tobacco=2]"^^xsd:string ;
    gufo:inheresIn :RipperRule15 ;
    a owl:NamedIndividual, :ExplanationComponentCharacteristic .

:RipperRule16
    gufo:isComponentOf :RipperExplanation ;
    a owl:NamedIndividual, :ExplanationComponent .

:RipperRule16Value
    gufo:hasQualityValue "[intubed=1 ^ icu=2]"^^xsd:string ;
    gufo:inheresIn :RipperRule16 ;
    a owl:NamedIndividual, :ExplanationComponentCharacteristic .

:RipperRule1ExplainsResultInstance46
    a owl:NamedIndividual, :ExplainsResultInstance ;
    :explainsInvolvesExplanationComponent :RipperRule01 ;
    :explainsInvolvesResultInstance :ResultInstance46 .

:RipperRule6ExplainsResultInstance28
    a owl:NamedIndividual, :ExplainsResultInstance ;
    :explainsInvolvesExplanationComponent :RipperRule06 ;
    :explainsInvolvesResultInstance :ResultInstance28 .

:RipperRule7ExplainsResultInstance15
    a owl:NamedIndividual, :ExplainsResultInstance ;
    :explainsInvolvesExplanationComponent :RipperRule07 ;
    :explainsInvolvesResultInstance :ResultInstance15 .

:RipperRulesAccuracy
    gufo:hasQualityValue 0.90 ;
    gufo:inheresIn :EvaluationRIPPERAccuracy ;
    a owl:NamedIndividual, :ExplanationAccuracy .

:Rules
    a owl:NamedIndividual, :ExplanationFormat ;
    rdfs:comment "Indicates that the explainable method generates explanations in the format of rules." .

:SPLIMEExplainsSVMModel
    a owl:NamedIndividual, :ExplainsModel ;
    :explainsModelInvolvesModel :SVMModel ;
    :explainsModelInvolvesModelExplanation :SPLimeExplanation .

:SPLimeEvaluation
    gufo:wasCreatedIn :EvaluateSPLIME ;
    a owl:NamedIndividual, :ExplanationEvaluation .

:SPLimeExplanation
    gufo:participatedIn :EvaluateSPLIME ;
    gufo:wasCreatedIn :ExplainSVMLIME ;
    a owl:NamedIndividual, :ModelExplanation .

:SPLimeExplanation01
    gufo:isComponentOf :SPLimeExplanation ;
    a owl:NamedIndividual, :ExplanationComponent .

:SPLimeExplanation01Value
    gufo:hasQualityValue """{'intubed=2': 0.7302359122759174,
 'icu=2': -0.22954003757272462,
 'pneumonia=1': 0.04581327864020495,
 'patient_type=2': -0.034584928434211695,
 'asthma=2': 0.027595011362469453,
 'age': 0.02738461930590004,
 'other_disease=1': -0.026795250312212974,
 'cardiovascular=2': 0.019499776159190345,
 'renal_chronic=2': -0.017185647822532412,
 'copd=1': -0.015029791025598985,
 'hypertension=1': 0.012109344746743541,
 'immunosuppression=2': -0.010143495665769735,
 'sex=1': -0.009535126637207039,
 'diabetes=1': -0.0029883123021770064,
 'tobacco=2': 0.0016895031607088214,
 'obesity=1': 0.001163529237239696,
 'exp number': 1}"""^^xsd:string ;
    gufo:inheresIn :SPLimeExplanation01 ;
    a owl:NamedIndividual, :ExplanationComponentCharacteristic .

:SPLimeExplanation02
    gufo:isComponentOf :SPLimeExplanation ;
    a owl:NamedIndividual, :ExplanationComponent .

:SPLimeExplanation02Value
    gufo:hasQualityValue """{'intubed=2': 0.7272498521085603,
 'icu=2': -0.2421863611446646,
 'pneumonia=1': 0.04253194088840385,
 'renal_chronic=2': -0.04082307044947787,
 'immunosuppression=2': -0.03780903346185646,
 'copd=1': -0.03181651896221923,
 'age': 0.023476161504144204,
 'patient_type=2': -0.01472961568828479,
 'diabetes=1': -0.01122094270293093,
 'obesity=1': -0.009858389349132319,
 'cardiovascular=2': 0.009525737521261932,
 'hypertension=1': 0.00924052022631108,
 'asthma=2': 0.00826332067373552,
 'sex=1': -0.005026340253797025,
 'tobacco=2': 0.0028567527217517245,
 'other_disease=2': 0.0005695780252155741,
 'exp number': 1}"""^^xsd:string ;
    gufo:inheresIn :SPLimeExplanation02 ;
    a owl:NamedIndividual, :ExplanationComponentCharacteristic .

:SPLimeExplanation03
    gufo:isComponentOf :SPLimeExplanation ;
    a owl:NamedIndividual, :ExplanationComponent .

:SPLimeExplanation03Value
    gufo:hasQualityValue """{'intubed=1': 0.6553617786618254,
 'icu=1': -0.2451102674364559,
 'renal_chronic=2': -0.07599107114491671,
 'pneumonia=1': 0.05209765097200194,
 'tobacco=1': -0.035714286774753336,
 'cardiovascular=2': 0.024268778740394372,
 'asthma=2': 0.02163447913495186,
 'age': 0.01943252669867966,
 'hypertension=2': -0.019300023723394552,
 'immunosuppression=2': -0.01357399240165284,
 'patient_type=2': -0.009912440527736332,
 'obesity=1': 0.00989801823162346,
 'other_disease=2': 0.006915059486896542,
 'diabetes=1': -0.00682619817619423,
 'copd=2': 0.0033162724258061545,
 'sex=2': 0.0019108890933709247,
 'exp number': 2}"""^^xsd:string ;
    gufo:inheresIn :SPLimeExplanation03 ;
    a owl:NamedIndividual, :ExplanationComponentCharacteristic .

:SPLimeExplanation04
    gufo:isComponentOf :SPLimeExplanation ;
    a owl:NamedIndividual, :ExplanationComponent .

:SPLimeExplanation04Value
    gufo:hasQualityValue """{'intubed=2': 0.7057727742821465,
 'icu=2': -0.23763531949355285,
 'pneumonia=1': 0.04901037794450674,
 'cardiovascular=1': -0.04238624673910528,
 'patient_type=2': -0.0228036323960163,
 'other_disease=1': -0.01820419544062246,
 'tobacco=1': -0.018155757223197164,
 'renal_chronic=1': 0.01671595321011683,
 'immunosuppression=1': -0.015370380829449186,
 'age': 0.015038212937832694,
 'copd=1': -0.013541457225898392,
 'sex=1': -0.012928745421242156,
 'asthma=1': -0.01223954829809454,
 'diabetes=1': -0.008036259015752074,
 'obesity=1': -0.005226248652916203,
 'hypertension=1': -0.0008443806814255352,
 'exp number': 3}"""^^xsd:string ;
    gufo:inheresIn :SPLimeExplanation04 ;
    a owl:NamedIndividual, :ExplanationComponentCharacteristic .

:SPLimeExplanation05
    gufo:isComponentOf :SPLimeExplanation ;
    a owl:NamedIndividual, :ExplanationComponent .

:SPLimeExplanation05Value
    gufo:hasQualityValue """{'intubed=2': 0.7249059880876344,
 'icu=2': -0.23506496954265338,
 'pneumonia=2': -0.0394402043900181,
 'patient_type=2': -0.02830830958544467,
 'immunosuppression=2': 0.027876847156680578,
 'cardiovascular=2': 0.0261611057578221,
 'tobacco=2': 0.02440373659248841,
 'asthma=2': 0.020537755319247064,
 'age': 0.019889050457562247,
 'hypertension=1': 0.015303023086232702,
 'copd=2': 0.013393110145669539,
 'renal_chronic=1': 0.012298246260305694,
 'diabetes=2': -0.010665702285202923,
 'sex=2': 0.010493478169157439,
 'obesity=2': 0.004463017322041727,
 'other_disease=2': -0.00021578332411475271,
 'exp number': 4}"""^^xsd:string ;
    gufo:inheresIn :SPLimeExplanation05 ;
    a owl:NamedIndividual, :ExplanationComponentCharacteristic .

:SVM
    dc:creator "Vladimir Vapnik"^^xsd:string ;
    dc:date "1963"^^xsd:date ;
    gufo:hasReifiedQualityValue :Classification, :Supervised, :Tabular ;
    a owl:NamedIndividual, :MLAlgorithm ;
    rdfs:label "Support Vector Machine"^^xsd:string .

:SVMAccuracyValue
    gufo:hasQualityValue 0.9 ;
    gufo:inheresIn :AccuracySpecifiesSVMEvaluation ;
    a owl:NamedIndividual, :MeasureValue .

:SVMAddressesClassification_exp1
    a owl:NamedIndividual, :Addresses ;
    :addressesInvolvesAlgorithm :SVM ;
    :addressesInvolvesGoal :ClassifyMortality_exp1 .

:SVMAddressesClassification_exp2
    a owl:NamedIndividual, :Addresses ;
    :addressesInvolvesAlgorithm :SVM ;
    :addressesInvolvesGoal :ClassifyMortality_exp2 .

:SVMEvaluation
    gufo:wasCreatedIn :EvaluateSVM ;
    a owl:NamedIndividual, :ModelEvaluation ;
    rdfs:comment "SVM evaluation using testing set."^^xsd:string .

:SVMKernelSetting
    gufo:participatedIn :TrainSVM ;
    a owl:NamedIndividual, :ParameterSetting ;
    rdfs:comment "Indicates the type of kernel used to train the SVM model."^^xsd:string .

:SVMKernelValue
    gufo:hasQualityValue "Linear"^^xsd:string ;
    gufo:inheresIn :SVMKernelSetting ;
    a owl:NamedIndividual, :ParameterSettingValue .

:SVMModel
    gufo:hasReifiedQualityValue :Inscrutable ;
    gufo:wasCreatedIn :TrainSVM ;
    a owl:NamedIndividual, :MLModel ;
    rdfs:comment "Fitted ML model generated in the train operation."^^xsd:string .

:SVMPython
    dc:creator "Scikit-learn: Machine Learning in Python, Pedregosa et al., JMLR 12, pp. 2825-2830, 2011."^^xsd:string ;
    gufo:isComponentOf :MLWorkflow, :PythonNotebook ;
    a owl:NamedIndividual, :MLImplementation ;
    rdfs:comment "Implementation of the Support Vector Machine Algorithm in the scikit-learn library in Python."^^xsd:string ;
    :executedBy :TrainSVM .

:SVMPythonFromLibrary
    dc:creator "Scikit-learn: Machine Learning in Python, Pedregosa et al., JMLR 12, pp. 2825-2830, 2011."^^xsd:string ;
    gufo:hasQualityValue "scikit-learn"^^xsd:string ;
    gufo:inheresIn :SVMPython ;
    a owl:NamedIndividual, :ImplementationLibrary .

:SVMPythonHasParameterTypeOfKernel
    a owl:NamedIndividual, :HasParameter ;
    :hasParameterInvolvesImplementation :SVMPython ;
    :hasParameterInvolvesParameter :TypeOfKernelParam .

:SVMPythonImplementsSVM
    a owl:NamedIndividual, :Implements ;
    :implementsInvolvesAlgorithm :SVM ;
    :implementsInvolvesImplementation :SVMPython .

:SVMSensitivityValue
    gufo:hasQualityValue 0.79 ;
    gufo:inheresIn :SensitivitySpecifiesSVMEvaluation ;
    a owl:NamedIndividual, :MeasureValue .

:SVMSpecificityValue
    gufo:hasQualityValue 0.9 ;
    gufo:inheresIn :SpecificitySpecifiesSVMEvaluation ;
    a owl:NamedIndividual, :MeasureValue .

:SVMTransparency
    gufo:hasQualityValue """SVM maps training examples to points in space so as to maximise the width of the gap between the two categories. New examples are then mapped into that same space and predicted to belong to a category based on which side of the gap they fall.

In addition to performing linear classification, SVMs can efficiently perform a non-linear classification using what is called the kernel trick, implicitly mapping their inputs into high-dimensional feature spaces.

When data are unlabelled, supervised learning is not possible, and an unsupervised learning approach is required, which attempts to find natural clustering of the data to groups, and then map new data to these formed groups."""^^rdfs:Literal ;
    gufo:inheresIn :SVM ;
    a owl:NamedIndividual, :AlgorithmTransparency .

:Sensitivity
    dc:creator "Jacob Yerushalmy"^^xsd:string ;
    dc:date "1947"^^xsd:date ;
    dc:rights "https://en.wikipedia.org/wiki/Sensitivity_and_specificity"^^xsd:string ;
    a owl:NamedIndividual, :EvaluationMeasure ;
    rdfs:comment """Sensitivity (True Positive rate) measures the proportion of positives that are correctly identified (i.e. the proportion of those who have some condition (affected) who are correctly identified as having the condition).
 In a diagnostic test, sensitivity is a measure of how well a test can identify true positives."""^^xsd:string ;
    rdfs:seeAlso "True Positive Rate, recall of the positive class, hit rate"^^xsd:string .

:SensitivitySpecifiesSVMEvaluation
    a owl:NamedIndividual, :SpecifiesModelEvaluation ;
    :specifiesInvolvesEvaluationMeasure :Sensitivity ;
    :specifiesInvolvesModelEvaluation :SVMEvaluation .

:Sex_Covid-19
    gufo:hasReifiedQualityValue :Categorical ;
    gufo:isComponentOf :Covid-19 ;
    a owl:NamedIndividual, :Feature ;
    rdfs:comment "SEX Identifies the sex of the patient."@en .

:Sex_Covid-19Test
    gufo:hasReifiedQualityValue :Categorical ;
    gufo:isComponentOf :Covid-19TestData ;
    a owl:NamedIndividual, :Feature ;
    rdfs:comment "SEX Identifies the sex of the patient."@en .

:Sex_Covid-19Test_categories
    gufo:hasQualityValue "1=woman, 2=man"^^xsd:string ;
    gufo:inheresIn :Sex_Covid-19Test ;
    a owl:NamedIndividual, :Categories .

:Sex_Covid-19Train
    gufo:hasReifiedQualityValue :Categorical ;
    gufo:isComponentOf :Covid-19TrainData ;
    a owl:NamedIndividual, :Feature ;
    rdfs:comment "SEX Identifies the sex of the patient."@en .

:Sex_Covid-19Train_1
    gufo:hasQualityValue 3123 ;
    gufo:inheresIn :Sex_Covid-19Train ;
    a owl:NamedIndividual, :CategoryQuantity .

:Sex_Covid-19Train_2
    gufo:hasQualityValue 3492 ;
    gufo:inheresIn :Sex_Covid-19Train ;
    a owl:NamedIndividual, :CategoryQuantity .

:Sex_Covid-19Train_categories
    gufo:hasQualityValue "1=woman, 2=man"^^xsd:string ;
    gufo:inheresIn :Sex_Covid-19Train ;
    a owl:NamedIndividual, :Categories .

:Sex_Covid-19_1
    gufo:hasQualityValue 279490 ;
    gufo:inheresIn :Sex_Covid-19 ;
    a owl:NamedIndividual, :CategoryQuantity .

:Sex_Covid-19_2
    gufo:hasQualityValue 287112 ;
    gufo:inheresIn :Sex_Covid-19 ;
    a owl:NamedIndividual, :CategoryQuantity .

:Sex_Covid-19_categories
    gufo:hasQualityValue "1=woman, 2=man"^^xsd:string ;
    gufo:inheresIn :Sex_Covid-19 ;
    a owl:NamedIndividual, :Categories .

:Software
    a gufo:Kind, owl:Class, owl:NamedIndividual ;
    rdfs:comment "Software is implemented computer programs, procedures, scripts or rules with associated documentation, possibly constituting an organized environment, stored in read/write memory for the purpose of being executed within a computer system."@en ;
    rdfs:label "Software"@en ;
    rdfs:subClassOf gufo:FunctionalComplex .

:Source
    a gufo:SubKind, owl:Class, owl:NamedIndividual ;
    rdfs:comment "Indicates the source of the dataset, for example, the book or the website."@en ;
    rdfs:label "Source"@en ;
    rdfs:subClassOf :DataSource .

:SourceName
    a gufo:SubKind, owl:Class, owl:NamedIndividual ;
    rdfs:comment "Indicates the source name of the dataset."@en ;
    rdfs:label "SourceName"@en ;
    rdfs:subClassOf :DataSource .

:Specificity
    dc:creator "Jacob Yerushalmy"^^xsd:string ;
    dc:date "1947"^^xsd:date ;
    dc:rights "https://en.wikipedia.org/wiki/Sensitivity_and_specificity"^^xsd:string ;
    a owl:NamedIndividual, :EvaluationMeasure ;
    rdfs:comment "Specificity (True Negative rate) measures the proportion of negatives that are correctly identified (i.e. the proportion of those who do not have the condition (unaffected) who are correctly identified as not having the condition)."^^xsd:string ;
    rdfs:seeAlso "recall of the negative class, selectivity or true negative rate"^^xsd:string .

:SpecificitySpecifiesSVMEvaluation
    a owl:NamedIndividual, :SpecifiesModelEvaluation ;
    :specifiesInvolvesEvaluationMeasure :Specificity ;
    :specifiesInvolvesModelEvaluation :SVMEvaluation .

:SpecifiesMeasure
    a gufo:Kind, owl:Class, owl:NamedIndividual ;
    rdfs:comment "Relator that indicates that the Goal of the study specifies which evaluation measures are adequate to evaluate the Machine Learning Model."@en ;
    rdfs:label "SpecifiesMeasure"@en ;
    rdfs:subClassOf gufo:Relator, [
        a owl:Restriction ;
        owl:minQualifiedCardinality "1"^^xsd:nonNegativeInteger ;
        owl:onClass :EvaluationMeasure ;
        owl:onProperty gufo:mediates
    ], [
        a owl:Restriction ;
        owl:minQualifiedCardinality "1"^^xsd:nonNegativeInteger ;
        owl:onClass :Goal ;
        owl:onProperty gufo:mediates
    ] .

:SpecifiesModelEvaluation
    a gufo:Kind, owl:Class, owl:NamedIndividual ;
    rdfs:comment "Relator that indicates that the evaluation measures specify the model evaluation."@en ;
    rdfs:label "SpecifiesModelEvaluation"@en ;
    rdfs:subClassOf gufo:Relator, [
        a owl:Restriction ;
        owl:minQualifiedCardinality "1"^^xsd:nonNegativeInteger ;
        owl:onClass :EvaluationMeasure ;
        owl:onProperty gufo:mediates
    ], [
        a owl:Restriction ;
        owl:minQualifiedCardinality "1"^^xsd:nonNegativeInteger ;
        owl:onClass :ModelEvaluation ;
        owl:onProperty gufo:mediates
    ], [
        a owl:Restriction ;
        owl:onClass :ModelEvaluationCharacteristic ;
        owl:onProperty [
            owl:inverseOf gufo:inheresIn
        ] ;
        owl:qualifiedCardinality "1"^^xsd:nonNegativeInteger
    ] .

:SpecifiesParameter
    a gufo:Kind, owl:Class, owl:NamedIndividual ;
    rdfs:comment "Relator that indicates that the ParameterSetting is specified by the Parameter."@en ;
    rdfs:label "SpecifiesParameter"@en ;
    rdfs:subClassOf gufo:Relator, [
        a owl:Restriction ;
        owl:minQualifiedCardinality "1"^^xsd:nonNegativeInteger ;
        owl:onClass :Parameter ;
        owl:onProperty gufo:mediates
    ], [
        a owl:Restriction ;
        owl:minQualifiedCardinality "1"^^xsd:nonNegativeInteger ;
        owl:onClass :ParameterSetting ;
        owl:onProperty gufo:mediates
    ] .

:Split
    gufo:hasReifiedQualityValue :SplitData ;
    a owl:NamedIndividual, :PreprocessingAlgorithm ;
    rdfs:comment "Split data into train and test sets."@en .

:SplitData
    a owl:NamedIndividual, :PreprocessingTechnique ;
    rdfs:comment "Indicates that the preprocessing technique is related to splitting the data into train and test sets." .

:SplitDataHasParameterTestSize
    a owl:NamedIndividual, :HasParameter ;
    :hasParameterInvolvesImplementation :SplitPython ;
    :hasParameterInvolvesParameter :TestSizeParam .

:SplitPython
    dc:creator "Scikit-learn: Machine Learning in Python, Pedregosa et al., JMLR 12, pp. 2825-2830, 2011."^^xsd:string ;
    gufo:isComponentOf :MLWorkflow, :PythonNotebook ;
    a owl:NamedIndividual, :PreprocessImplementation ;
    rdfs:comment "Implementation of split function  in Python to split a dataset into train and test  sets."^^xsd:string ;
    :executedBy :PreprocessCovid .

:SplitPythonFromLibrary
    dc:creator "Scikit-learn: Machine Learning in Python, Pedregosa et al., JMLR 12, pp. 2825-2830, 2011."^^xsd:string ;
    gufo:hasQualityValue "scikit-learn"^^xsd:string ;
    gufo:inheresIn :SplitPython ;
    a owl:NamedIndividual, :ImplementationLibrary .

:SplitPythonImplementsSplit
    a owl:NamedIndividual, :Implements ;
    :implementsInvolvesAlgorithm :Split ;
    :implementsInvolvesImplementation :SplitPython .

:Static
    a owl:NamedIndividual, :ExplanationInteraction ;
    rdfs:comment "Indicates that the explainable method generates static explanations." .

:Study
    a owl:Class ;
    rdfs:subClassOf gufo:Event .

:SuitableMeasurement
    a gufo:SubKind, owl:Class, owl:NamedIndividual ;
    rdfs:comment "Suitable measurements for the goal, for example, sensitivity and specificity for diagnosis."@en ;
    rdfs:label "SuitableMeasurement"@en ;
    rdfs:subClassOf :GoalCharacteristic .

:Supervised
    a owl:NamedIndividual, :LearningType ;
    rdfs:comment "Indicates that the ML algorithm performs supervised learning (labeled data)." .

:Tabular
    a owl:NamedIndividual, :DataType .

:TestData
    a gufo:Role, owl:Class, owl:NamedIndividual ;
    rdfs:comment "Part of preprocessed data that has the role to be used by the Test(predict) operation. "@en ;
    rdfs:label "TestData"@en ;
    rdfs:subClassOf :PreprocessedData ;
    owl:disjointWith :TrainData .

:TestPredict
    a gufo:EventType, owl:NamedIndividual .

:TestPrediction
    gufo:participatedIn :EvaluateSVM ;
    gufo:wasCreatedIn :PredictTest ;
    a owl:NamedIndividual, :Result ;
    rdfs:comment "Result predicted using the fitted SVM in the test set."^^xsd:string .

:TestSizeParam
    a owl:NamedIndividual, :Parameter ;
    rdfs:comment "Parameter to indicate the size of the test set to split the original dataset."@en .

:TestSizeSetting
    gufo:participatedIn :PreprocessCovid ;
    a owl:NamedIndividual, :ParameterSetting ;
    rdfs:comment "Indicates the size of the test set to split the original dataset."^^xsd:string .

:TestSizeSpecifiesTestSizeSetting
    a owl:NamedIndividual, :SpecifiesParameter ;
    :specifiesInvolvesParameter :TestSizeParam ;
    :specifiesInvolvesParameterSetting :TestSizeSetting .

:TestSizeValue
    gufo:hasQualityValue "0.3"^^xsd:string ;
    gufo:inheresIn :TestSizeSetting ;
    a owl:NamedIndividual, :ParameterSettingValue .

:Text
    a owl:NamedIndividual, :DataType .

:Tobacco_Covid-19
    gufo:hasReifiedQualityValue :Categorical ;
    gufo:isComponentOf :Covid-19 ;
    a owl:NamedIndividual, :Feature ;
    rdfs:comment "TOBACCO Identify if the patient has a smoking habit."@en .

:Tobacco_Covid-19Test
    gufo:hasReifiedQualityValue :Categorical ;
    gufo:isComponentOf :Covid-19TestData ;
    a owl:NamedIndividual, :Feature ;
    rdfs:comment "TOBACCO Identify if the patient has a smoking habit."@en .

:Tobacco_Covid-19Test_categories
    gufo:hasQualityValue "1 = Yes , 2 = No"^^xsd:string ;
    gufo:inheresIn :Tobacco_Covid-19Test ;
    a owl:NamedIndividual, :Categories .

:Tobacco_Covid-19Train
    gufo:hasReifiedQualityValue :Categorical ;
    gufo:isComponentOf :Covid-19TrainData ;
    a owl:NamedIndividual, :Feature ;
    rdfs:comment "TOBACCO Identify if the patient has a smoking habit."@en .

:Tobacco_Covid-19Train_1
    gufo:hasQualityValue 502 ;
    gufo:inheresIn :Tobacco_Covid-19Train ;
    a owl:NamedIndividual, :CategoryQuantity .

:Tobacco_Covid-19Train_2
    gufo:hasQualityValue 6113 ;
    gufo:inheresIn :Tobacco_Covid-19Train ;
    a owl:NamedIndividual, :CategoryQuantity .

:Tobacco_Covid-19Train_categories
    gufo:hasQualityValue "1 = Yes , 2 = No"^^xsd:string ;
    gufo:inheresIn :Tobacco_Covid-19Train ;
    a owl:NamedIndividual, :Categories .

:Tobacco_Covid-19_1
    gufo:hasQualityValue 48017 ;
    gufo:inheresIn :Tobacco_Covid-19 ;
    a owl:NamedIndividual, :CategoryQuantity .

:Tobacco_Covid-19_2
    gufo:hasQualityValue 516678 ;
    gufo:inheresIn :Tobacco_Covid-19 ;
    a owl:NamedIndividual, :CategoryQuantity .

:Tobacco_Covid-19_Null
    gufo:hasQualityValue 1907 ;
    gufo:inheresIn :Tobacco_Covid-19 ;
    a owl:NamedIndividual, :NumberNulls .

:Tobacco_Covid-19_categories
    gufo:hasQualityValue "1 = Yes, 2 = No"^^xsd:string ;
    gufo:inheresIn :Tobacco_Covid-19 ;
    a owl:NamedIndividual, :Categories .

:Train
    a gufo:EventType, owl:Class, owl:NamedIndividual ;
    rdfs:comment "Specific type of operation that train the Machine Learning model, executing the ML Algorithm implementation."@en ;
    rdfs:label "Train"@en ;
    rdfs:subClassOf :Operation, [
        a owl:Restriction ;
        owl:onProperty gufo:historicallyDependsOn ;
        owl:someValuesFrom :Preprocess
    ], [
        a owl:Restriction ;
        owl:onProperty [
            owl:inverseOf gufo:participatedIn
        ] ;
        owl:someValuesFrom :TrainData
    ], [
        a owl:Restriction ;
        owl:minQualifiedCardinality "1"^^xsd:nonNegativeInteger ;
        owl:onClass :MLImplementation ;
        owl:onProperty [
            owl:inverseOf gufo:participatedIn
        ]
    ], [
        a owl:Restriction ;
        owl:onClass :MLModel ;
        owl:onProperty [
            owl:inverseOf gufo:wasCreatedIn
        ] ;
        owl:qualifiedCardinality "1"^^xsd:nonNegativeInteger
    ] .

:TrainData
    a gufo:Role, owl:Class, owl:NamedIndividual ;
    rdfs:comment "Part of preprocessed data that has the role to be used by the Train operation. "@en ;
    rdfs:label "TrainData"@en ;
    rdfs:subClassOf :PreprocessedData .

:TrainPrediction_exp1
    gufo:participatedIn :ExplainSVMRIPPER ;
    gufo:wasCreatedIn :PredictTrain_exp1 ;
    a owl:NamedIndividual, :Result ;
    rdfs:comment "Result predicted using the fitted SVM in the train set."^^xsd:string .

:TrainSVM
    dc:creator "Patricia"^^xsd:string ;
    gufo:historicallyDependsOn :PreprocessCovid ;
    gufo:isEventProperPartOf :MLWorkflow_exec ;
    a owl:NamedIndividual, :Train ;
    rdfs:comment "Train Support Vector Machine using train data."^^xsd:string .

:TransformData
    a owl:NamedIndividual, :PreprocessingTechnique ;
    rdfs:comment "Indicates that the preprocessing technique is related to transforming the data, for example renaming columns or encoding labels." .

:Transparent
    a owl:NamedIndividual, :Interpretability ;
    rdfs:comment "Indicates that the ML algorithm is transparent." .

:TypeOfKernelParam
    a owl:NamedIndividual, :Parameter ;
    rdfs:comment "Parameter to indicate the type of kernel of SVM  (linear’, ‘poly’, ‘rbf’, ‘sigmoid’, ‘precomputed’)"@en .

:Unfaithful
    a owl:NamedIndividual, :ExplanationFidelity ;
    rdfs:comment "Indicates if the explanation if unfaithfull to the underlying ML model." .

:Unsupervised
    a owl:NamedIndividual, :LearningType ;
    rdfs:comment "Indicates that the ML algorithm performs unsupervised learning (uses unlabeled data)." .

:WFExecution
    a gufo:EventType, owl:Class, owl:NamedIndividual ;
    rdfs:comment "Workflow execution (WFExecution) is complex process composed of a series of operations. It executes the implementations of  operations by executing Workflows, which organizes sequentially the implementations of these operations."@en ;
    rdfs:label "WFExecution"@en ;
    rdfs:subClassOf gufo:Event, [
        a owl:Restriction ;
        owl:onProperty gufo:isEventProperPartOf ;
        owl:someValuesFrom :Experiment
    ], [
        a owl:Restriction ;
        owl:onProperty [
            owl:inverseOf gufo:isEventProperPartOf
        ] ;
        owl:someValuesFrom :Operation
    ], [
        a owl:Restriction ;
        owl:onProperty [
            owl:inverseOf gufo:participatedIn
        ] ;
        owl:someValuesFrom :Workflow
    ] .

:Workflow
    a gufo:Kind, owl:Class, owl:NamedIndividual ;
    rdfs:comment "Workflow is a complex structure thais composed of series of implementations that need to be completed sequentially. It can be, for example, a workflow for the ML process and a workflow for the explanation."@en ;
    rdfs:label "Workflow"@en ;
    rdfs:subClassOf gufo:FunctionalComplex .

:addressesInvolvesAlgorithm
    a owl:AsymmetricProperty, owl:IrreflexiveProperty, owl:ObjectProperty ;
    rdfs:domain :Addresses ;
    rdfs:range :Algorithm ;
    rdfs:subPropertyOf gufo:mediates .

:addressesInvolvesGoal
    a owl:AsymmetricProperty, owl:IrreflexiveProperty, owl:ObjectProperty ;
    rdfs:domain :Addresses ;
    rdfs:range :Goal ;
    rdfs:subPropertyOf gufo:mediates .

:assessesInvolvesModel
    a owl:AsymmetricProperty, owl:IrreflexiveProperty, owl:ObjectProperty ;
    rdfs:domain :Assesses ;
    rdfs:range :MLModel ;
    rdfs:subPropertyOf gufo:mediates .

:assessesInvolvesModelEvaluation
    a owl:AsymmetricProperty, owl:IrreflexiveProperty, owl:ObjectProperty ;
    rdfs:domain :Assesses ;
    rdfs:range :ModelEvaluation ;
    rdfs:subPropertyOf gufo:mediates .

:callsInvolvesMLModel
    a owl:AsymmetricProperty, owl:IrreflexiveProperty, owl:ObjectProperty ;
    rdfs:domain :Calls ;
    rdfs:range :MLModel ;
    rdfs:subPropertyOf gufo:mediates .

:callsInvolvesPredictImplementation
    a owl:AsymmetricProperty, owl:IrreflexiveProperty, owl:ObjectProperty ;
    rdfs:domain :Calls ;
    rdfs:range :PredictImplementation ;
    rdfs:subPropertyOf gufo:mediates .

:correlates
    a owl:AsymmetricProperty, owl:IrreflexiveProperty, owl:ObjectProperty ;
    rdfs:domain :Correlates ;
    rdfs:range :Feature ;
    rdfs:subPropertyOf gufo:mediates .

:evaluatesInvolvesExplanationComponent
    a owl:AsymmetricProperty, owl:IrreflexiveProperty, owl:ObjectProperty ;
    rdfs:domain :EvaluatesExplanationComponent ;
    rdfs:range :ExplanationComponent ;
    rdfs:subPropertyOf gufo:mediates .

:evaluatesInvolvesExplanationComponentEvaluation
    a owl:AsymmetricProperty, owl:IrreflexiveProperty, owl:ObjectProperty ;
    rdfs:domain :EvaluatesExplanationComponent ;
    rdfs:range :ExplanationComponentEvaluation ;
    rdfs:subPropertyOf gufo:mediates .

:executedBy
    a owl:AsymmetricProperty, owl:IrreflexiveProperty, owl:ObjectProperty ;
    rdfs:domain :Implementation ;
    rdfs:range :Operation ;
    rdfs:subPropertyOf gufo:participatedIn .

:explainsInvolvesExplanationComponent
    a owl:AsymmetricProperty, owl:IrreflexiveProperty, owl:ObjectProperty ;
    rdfs:domain :ExplainsResultInstance ;
    rdfs:range :ExplanationComponent ;
    rdfs:subPropertyOf gufo:mediates .

:explainsInvolvesResultInstance
    a owl:AsymmetricProperty, owl:IrreflexiveProperty, owl:ObjectProperty ;
    rdfs:domain :ExplainsResultInstance ;
    rdfs:range :ResultInstance ;
    rdfs:subPropertyOf gufo:mediates .

:explainsModelInvolvesModel
    a owl:AsymmetricProperty, owl:IrreflexiveProperty, owl:ObjectProperty ;
    rdfs:domain :ExplainsModel ;
    rdfs:range :MLModel ;
    rdfs:subPropertyOf gufo:mediates .

:explainsModelInvolvesModelExplanation
    a owl:AsymmetricProperty, owl:IrreflexiveProperty, owl:ObjectProperty ;
    rdfs:domain :ExplainsModel ;
    rdfs:range :ModelExplanation ;
    rdfs:subPropertyOf gufo:mediates .

:hasMeasure
    a gufo:Kind, owl:NamedIndividual .

:hasMeasureInvolvesEvaluateModelImplementation
    a owl:AsymmetricProperty, owl:IrreflexiveProperty, owl:ObjectProperty ;
    rdfs:domain :HasMeasure ;
    rdfs:range :EvaluateModelImplementation ;
    rdfs:subPropertyOf gufo:mediates .

:hasMeasureInvolvesMeasure
    a owl:AsymmetricProperty, owl:IrreflexiveProperty, owl:ObjectProperty ;
    rdfs:domain :HasMeasure ;
    rdfs:range :EvaluationMeasure ;
    rdfs:subPropertyOf gufo:mediates .

:hasParameterInvolvesImplementation
    a owl:AsymmetricProperty, owl:IrreflexiveProperty, owl:ObjectProperty ;
    rdfs:domain :HasParameter ;
    rdfs:range :Implementation ;
    rdfs:subPropertyOf gufo:mediates .

:hasParameterInvolvesParameter
    a owl:AsymmetricProperty, owl:IrreflexiveProperty, owl:ObjectProperty ;
    rdfs:domain :HasParameter ;
    rdfs:range :Parameter ;
    rdfs:subPropertyOf gufo:mediates .

:implementsInvolvesAlgorithm
    a owl:AsymmetricProperty, owl:IrreflexiveProperty, owl:ObjectProperty ;
    rdfs:domain :Implements ;
    rdfs:range :Algorithm ;
    rdfs:subPropertyOf gufo:mediates .

:implementsInvolvesImplementation
    a owl:AsymmetricProperty, owl:IrreflexiveProperty, owl:ObjectProperty ;
    rdfs:domain :Implements ;
    rdfs:range :Implementation ;
    rdfs:subPropertyOf gufo:mediates .

:specifiesInvolvesEvaluationMeasure
    a owl:AsymmetricProperty, owl:IrreflexiveProperty, owl:ObjectProperty ;
    rdfs:domain :SpecifiesModelEvaluation ;
    rdfs:range :EvaluationMeasure ;
    rdfs:subPropertyOf gufo:mediates .

:specifiesInvolvesModelEvaluation
    a owl:AsymmetricProperty, owl:IrreflexiveProperty, owl:ObjectProperty ;
    rdfs:domain :SpecifiesModelEvaluation ;
    rdfs:range :ModelEvaluation ;
    rdfs:subPropertyOf gufo:mediates .

:specifiesInvolvesParameter
    a owl:AsymmetricProperty, owl:IrreflexiveProperty, owl:ObjectProperty ;
    rdfs:domain :SpecifiesParameter ;
    rdfs:range :Parameter ;
    rdfs:subPropertyOf gufo:mediates .

:specifiesInvolvesParameterSetting
    a owl:AsymmetricProperty, owl:IrreflexiveProperty, owl:ObjectProperty ;
    rdfs:domain :SpecifiesParameter ;
    rdfs:range :ParameterSetting ;
    rdfs:subPropertyOf gufo:mediates .

:specifiesMeasureInvolvesGoal
    a owl:AsymmetricProperty, owl:IrreflexiveProperty, owl:ObjectProperty ;
    rdfs:domain :SpecifiesMeasure ;
    rdfs:range :Goal ;
    rdfs:subPropertyOf gufo:mediates .

:specifiesMeasureInvolvesMeasure
    a owl:AsymmetricProperty, owl:IrreflexiveProperty, owl:ObjectProperty ;
    rdfs:domain :SpecifiesMeasure ;
    rdfs:range :EvaluationMeasure ;
    rdfs:subPropertyOf gufo:mediates .

[]
    a owl:AllDisjointClasses ;
    owl:members (:Algorithm
        :Data
        :EvaluationMeasure
        :ExplanationComponent
        :ExplanationComponentEvaluation
        :Feature
        :Goal
        :Implementation
        :Parameter
        :ParameterSetting
        :ResultInstance
        :Software
        :Workflow
    ) .

[]
    a owl:AllDisjointClasses ;
    owl:members (:AlgorithmCharacteristic
        :DataCharacteristic
        :ExperimentCharacteristic
        :ExplanationComponentEvaluationCharacteristic
        :GoalCharacteristic
        :ImplementationCharacteristic
        :ModelCharacteristic
        :ModelEvaluationCharacteristic
        :ParameterSettingCharacteristic
    ) .

[]
    a owl:AllDisjointClasses ;
    owl:members (:EvaluateExplanation
        :EvaluateModel
        :Explain
        :Predict
        :Preprocess
        :Train
    ) .

[]
    a owl:AllDisjointClasses ;
    owl:members (:Explanation
        :ExplanationEvaluation
        :MLModel
        :ModelEvaluation
        :PreprocessedData
        :Result
    ) .

